More work on pi calculus.

coq/MPST.v
@@ -2,6 +2,7 @@ Require Import Coq.Logic.JMeq.
 Require Import Coq.Arith.Arith.
 Require Import Coq.Classes.RelationClasses.
 Require Import Coq.Arith.PeanoNat.
+Require Import Coq.Program.Tactics.
 
 Require Export Expression.
 Require Export TypedExpression.
@@ -23,7 +24,7 @@ Module MPST (E : Expression) (TE : TypedExpression E) (STE : SoundlyTypedExpress
             | S m => S (ξ m)
             end.
 
-  Lemma RenamingUpExt : forall (ξ1 ξ2 : nat -> nat),
+    Lemma RenamingUpExt : forall (ξ1 ξ2 : nat -> nat),
       (forall n, ξ1 n = ξ2 n)
       -> forall n, RenamingUp ξ1 n = RenamingUp ξ2 n.
   Proof.
@@ -38,1030 +39,1311 @@ Module MPST (E : Expression) (TE : TypedExpression E) (STE : SoundlyTypedExpress
   Qed.
   Hint Resolve IdRenamingUp : PiC.
   Hint Rewrite IdRenamingUp : PiC.
-  
-  Inductive Chan : Set :=
-    ChanVar : nat -> Chan
-  | Session : nat -> Role -> Chan.
-  Hint Constructors Chan : PiC.
 
-  Lemma ChanEqDec : forall χ1 χ2 : Chan, {χ1 = χ2} + {χ1 <> χ2}.
-  Proof.
-    decide equality; auto with PiC; apply Nat.eq_dec.
-  Qed.
-  Hint Resolve ChanEqDec : PiC.
-  Definition ChanRename : Chan -> (nat -> nat) -> Chan :=
-    fun χ ξ => match χ with
-            | ChanVar n => ChanVar (ξ n)
-            | Session _ _ => χ
-            end.
-  Notation "χ ⟨ch| ξ ⟩" := (ChanRename χ ξ) (at level 15).
+  Inductive GSType' : Set :=
+    GEndType : GSType'
+  | GSendType : Role -> ExprTyp -> GSType -> GSType'
+  | GRecvType : Role -> ExprTyp -> GSType -> GSType'
+  | GEChoiceType : Role -> GSType -> GSType'
+  | GIChoiceType : Role -> GSType -> GSType -> GSType'
+  with GSType : Set :=
+    Gμ : GSType' -> GSType
+  | GSTypeVar : nat -> GSType
+  | GPlain : GSType' -> GSType.
+  Hint Constructors GSType : PiC.
+  Hint Constructors GSType' : PiC.
 
-  Lemma ChanIdRenaming : forall χ : Chan, χ ⟨ch| IdRenaming⟩ = χ.
-  Proof.
-    induction χ; auto.
-  Qed.
-  Hint Resolve ChanIdRenaming : PiC.
-  Hint Rewrite ChanIdRenaming : PiC.
+  Section GSTypeInd.
+    Variable P : GSType' -> Prop.
+    Variable Q : GSType -> Prop.
 
-  Lemma ChanRenameExt : forall (χ : Chan) (ξ1 ξ2 : nat -> nat),
-      (forall n, ξ1 n = ξ2 n)
-      -> χ ⟨ch| ξ1⟩ = χ ⟨ch| ξ2⟩.
-  Proof.
-    intros χ ξ1 ξ2 ext_eq; induction χ; simpl; auto.
-  Qed.
-  Hint Resolve ChanRenameExt : PiC.
-  Hint Rewrite ChanRenameExt : PiC.
+    Variable EndCase : P (GEndType).
+    Variable VarCase : forall n, Q (GSTypeVar n).
+    Variable SendCase : forall p τ T, Q T -> P (GSendType p τ T).
+    Variable RecvCase : forall p τ T, Q T -> P (GRecvType p τ T).
+    Variable EChoiceCase : forall p T, Q T -> P (GEChoiceType p T).
+    Variable IChoiceCase : forall p T1 T2, Q T1 -> Q T2 -> P (GIChoiceType p T1 T2).
+    Variable μCase : forall T, P T -> Q (Gμ T).
+    Variable PlainCase : forall T, P T -> Q (GPlain T).
 
-  Definition ChanSessionRename : Chan -> (nat -> nat) -> Chan :=
-    fun χ ξ => match χ with
-            | ChanVar _ => χ
-            | Session n p => Session (ξ n) p
-            end.
-  Notation "χ ⟨chs| ξ ⟩" := (ChanSessionRename χ ξ) (at level 15).
-  
-  Lemma ChanIdSessionRenaming : forall χ : Chan, χ ⟨chs|IdRenaming⟩ = χ.
-  Proof.
-    intro χ; induction χ; auto.
-  Qed.
-  Hint Resolve ChanIdSessionRenaming : PiC.
-  Hint Rewrite ChanIdSessionRenaming : PiC.
-
-  Lemma ChanSessionRenameExt : forall (χ : Chan) (ξ1 ξ2 : nat -> nat),
-      (forall n, ξ1 n = ξ2 n)
-      -> χ ⟨chs| ξ1⟩ = χ ⟨chs| ξ2⟩.
-  Proof.
-    intros χ ξ1 ξ2 ext_eq; destruct χ; simpl; auto.
-    rewrite ext_eq; reflexivity.
-  Qed.
-  Hint Resolve ChanSessionRenameExt : PiC.
-  Hint Rewrite ChanSessionRenameExt : PiC.
-
-  Definition ChanSubstUp : (nat -> Chan) -> nat -> Chan :=
-    fun σ n => match n with
-            | 0 => ChanVar 0
-            | S m => σ m ⟨ch| S⟩
-            end.
-  Lemma ChanSubstUpExt : forall (σ1 σ2 : nat -> Chan),
-      (forall n, σ1 n = σ2 n)
-      -> forall n, ChanSubstUp σ1 n = ChanSubstUp σ2 n.
-  Proof.
-    intros σ1 σ2 ext_eq n; destruct n; simpl; [|rewrite ext_eq]; reflexivity.
-  Qed.
-  Hint Resolve ChanSubstUpExt : PiC.
-  Hint Rewrite ChanSubstUpExt : PiC.
-  
-  Definition ChanSubst : Chan -> (nat -> Chan) -> Chan :=
-    fun χ σ => match χ with
-            | ChanVar n => (σ n)
-            | Session _ _ => χ
-            end.
-  Notation "χ [ch| σ ]" := (ChanSubst χ σ) (at level 15).
-
-  Definition ChanIdSubst : nat -> Chan := fun n => ChanVar n.
-  Lemma ChanIdSubstSpec : forall χ : Chan, χ [ch| ChanIdSubst] = χ.
-  Proof.
-    induction χ; auto.
-  Qed.
-  Hint Resolve ChanIdSubstSpec : PiC.
-  Hint Rewrite ChanIdSubstSpec : PiC.
-
-  Lemma ChanSubstIdUp : forall n, ChanSubstUp ChanIdSubst n = ChanIdSubst n.
-  Proof.
-    intro n; induction n; simpl; auto.
-  Qed.
-  Hint Resolve ChanSubstIdUp : PiC.
-  Hint Rewrite ChanSubstIdUp : PiC.
-
-  Lemma ChanSubstExt : forall (χ : Chan) (σ1 σ2 : nat -> Chan),
-      (forall n, σ1 n = σ2 n)
-      -> χ [ch| σ1] = χ [ch| σ2].
-  Proof.
-    intros χ σ1 σ2 ext_eq; induction χ; simpl; auto.
-  Qed.
-  Hint Resolve ChanSubstExt : PiC.
-  Hint Rewrite ChanSubstExt : PiC.
-
-  (* We only support binary choices. *)
-  Inductive SessionType : Set :=
-    EndType : SessionType
-  | TypeVar : nat -> SessionType
-  | μ : SessionType -> SessionType
-  | EChoice : Role -> SessionType -> SessionType
-  | IChoice : Role -> SessionType -> SessionType -> SessionType
-  | SendT : Role -> SessionType -> SessionType -> SessionType
-  | ReceiveT : Role -> SessionType -> SessionType -> SessionType
-  | SendDT : Role -> ExprTyp -> SessionType -> SessionType
-  | ReceiveDT : Role -> ExprTyp -> SessionType -> SessionType.
-  Hint Constructors SessionType : PiC.
-  Definition SessionTypeEqDec : forall S1 S2 : SessionType, {S1 = S2} + {S1 <> S2}.
-  Proof.
-    intros S1 S2; decide equality; auto with PiC.
-    apply Nat.eq_dec.
-    all: apply ExprTypEqDec.
-  Qed.
-
-  Fixpoint SessionTypeRename (S : SessionType) (ξ : nat -> nat) : SessionType :=
-    match S with
-    | EndType => EndType
-    | TypeVar n => TypeVar (ξ n)
-    | μ S' => μ (SessionTypeRename S' (RenamingUp ξ))
-    | EChoice p S' => EChoice p (SessionTypeRename S' ξ)
-    | IChoice p S1 S2 => IChoice p (SessionTypeRename S1 ξ) (SessionTypeRename S2 ξ)
-    | SendT p S1 S2 => SendT p (SessionTypeRename S1 ξ) (SessionTypeRename S2 ξ)
-    | ReceiveT p S1 S2 => ReceiveT p (SessionTypeRename S1 ξ) (SessionTypeRename S2 ξ)
-    | SendDT p τ S' => SendDT p τ (SessionTypeRename S' ξ)
-    | ReceiveDT p τ S' => ReceiveDT p τ (SessionTypeRename S' ξ)
-    end.
-  Notation "S ⟨s| ξ ⟩" := (SessionTypeRename S ξ) (at level 15).
-
-  Lemma SessionTypeRenameExt : forall (S : SessionType) (ξ1 ξ2 : nat -> nat),
-      (forall n, ξ1 n = ξ2 n)
-      -> S ⟨s| ξ1⟩ = S ⟨s| ξ2⟩.
-  Proof.
-    intro S; induction S; intros ξ1 ξ2 ext_eq; simpl; auto.
-    1: rewrite IHS with (ξ2 := RenamingUp ξ2); auto.
-    apply RenamingUpExt; auto.
-    1,5,6: rewrite IHS with (ξ2 := ξ2); auto.
-    all: rewrite IHS1 with (ξ2 := ξ2); auto; rewrite IHS2 with (ξ2 := ξ2); auto.
-  Qed.
-  Hint Resolve SessionTypeRenameExt : PiC.
-  Hint Rewrite SessionTypeRenameExt : PiC.
-
-  Lemma SessionTypeIdRenamingSpec : forall S : SessionType, S ⟨s|IdRenaming⟩ = S.
-  Proof.
-    intro S; induction S; simpl; auto.
-    rewrite SessionTypeRenameExt with (ξ2 := IdRenaming).
-    rewrite IHS; reflexivity.
-    apply IdRenamingUp.
-    1,5,6: rewrite IHS; auto.
-    all: rewrite IHS1; rewrite IHS2; auto.
-  Qed.
-  Hint Resolve SessionTypeIdRenamingSpec : PiC.
-  Hint Rewrite SessionTypeIdRenamingSpec : PiC.
-
-  Definition SessionTypeSubstUp : (nat -> SessionType) -> nat -> SessionType :=
-    fun σ n => match n with
-            | 0 => TypeVar 0
-            | S n' => (σ n') ⟨s| S⟩
-            end.
-
-  Lemma SessionTypeSubstUpExt : forall (σ1 σ2 : nat -> SessionType),
-      (forall n : nat, σ1 n = σ2 n)
-      -> forall n : nat, SessionTypeSubstUp σ1 n = SessionTypeSubstUp σ2 n.
-  Proof.
-    intros σ1 σ2 ext_eq n.
-    unfold SessionTypeSubstUp; destruct n; auto.
-    rewrite ext_eq; reflexivity.
-  Qed.
-  Hint Resolve SessionTypeSubstUpExt : PiC.
-  Hint Rewrite SessionTypeSubstUpExt : PiC.
-  
-  Fixpoint SessionTypeSubst (S : SessionType) (σ : nat -> SessionType) : SessionType :=
-    match S with
-    | EndType => EndType
-    | TypeVar n => σ n
-    | μ S' => μ (SessionTypeSubst S' (SessionTypeSubstUp σ))
-    | EChoice p S' => EChoice p (SessionTypeSubst S' σ)
-    | IChoice p S1 S2 => IChoice p (SessionTypeSubst S1 σ) (SessionTypeSubst S2 σ)
-    | SendT p S1 S2 => SendT p (SessionTypeSubst S1 σ) (SessionTypeSubst S2 σ)
-    | ReceiveT p S1 S2 => ReceiveT p (SessionTypeSubst S1 σ) (SessionTypeSubst S2 σ)
-    | SendDT p τ S' => SendDT p τ (SessionTypeSubst S' σ)
-    | ReceiveDT p τ S' => ReceiveDT p τ (SessionTypeSubst S' σ)
-    end.
-  Notation "S [s| σ ]" := (SessionTypeSubst S σ) (at level 15).
-
-  Lemma SessionTypeSubstExt : forall (S : SessionType) (σ1 σ2 : nat -> SessionType),
-      (forall n, σ1 n = σ2 n)
-      -> S [s| σ1] = S [s| σ2].
-  Proof.
-    intro S; induction S; intros σ1 σ2 ext_eq; simpl; auto with PiC.
-    rewrite IHS with (σ2 := SessionTypeSubstUp σ2); auto.
-    apply SessionTypeSubstUpExt; auto.
-    1,5,6:rewrite IHS with (σ2 := σ2); auto.
-    all: rewrite IHS1 with (σ2 := σ2); auto; rewrite IHS2 with (σ2 := σ2); auto.
-  Qed.    
-  Hint Resolve SessionTypeSubstExt : PiC.
-  Hint Rewrite SessionTypeSubstExt : PiC.
-
-  Definition SessionTypeIdSubst : nat -> SessionType :=
-    fun n => TypeVar n.
-  Lemma SessionTypeIdSubstUp :
-    forall n, SessionTypeSubstUp SessionTypeIdSubst n = SessionTypeIdSubst n.
-  Proof.
-    intro n; induction n; unfold SessionTypeSubstUp; unfold SessionTypeIdSubst;
-      simpl; reflexivity.
-  Qed.
-  Hint Resolve SessionTypeIdSubstUp : PiC.
-  Hint Rewrite SessionTypeIdSubstUp : PiC.
-
-  Lemma SessionTypeIdSubstSpec : forall (S : SessionType),
-      S [s| SessionTypeIdSubst] = S.
-  Proof.
-    intro S; induction S; simpl; auto.
-    rewrite SessionTypeSubstExt with (σ2 := SessionTypeIdSubst);
-      [rewrite IHS; auto | apply SessionTypeIdSubstUp].
-    1,5,6:rewrite IHS; auto.
-    all: rewrite IHS1; rewrite IHS2; auto.
-  Qed.
-  Hint Resolve SessionTypeIdSubstSpec : PiC.
-  Hint Rewrite SessionTypeIdSubstSpec : PiC.
-
-  CoInductive SessionSubtype : SessionType -> SessionType -> Prop :=
-  | SubEnd : SessionSubtype (EndType) (EndType)
-  | SubVar : forall n : nat, SessionSubtype (TypeVar n) (TypeVar n)
-  | SubμL : forall S T : SessionType,
-      SessionSubtype (SessionTypeSubst S (fun n =>
-                                          match n with
-                                          | 0 => μ S
-                                          | S n' => TypeVar n'
-                                          end)) T
-      -> SessionSubtype (μ S) T
-  | SubμR : forall S T : SessionType,
-      SessionSubtype S (SessionTypeSubst T (fun n =>
-                                          match n with
-                                          | 0 => μ T
-                                          | S n' => TypeVar n'
-                                          end))
-      -> SessionSubtype S (μ T)
-  | SubEChoice : forall p S T,
-      SessionSubtype S T
-      -> SessionSubtype (EChoice p S) (EChoice p T)
-  | SubIChoice : forall p S1 S2 T1 T2,
-      SessionSubtype S1 T1
-      -> SessionSubtype S2 T2
-      -> SessionSubtype (IChoice p S1 S2) (IChoice p T1 T2)
-  | SubSend : forall p S1 S2 T1 T2,
-      SessionSubtype S1 T1
-      -> SessionSubtype S2 T2
-      -> SessionSubtype (SendT p S1 S2) (SendT p T1 T2)
-  | SubReceive : forall p S1 S2 T1 T2,
-      SessionSubtype T1 S1 (* Note Contravariance! *)
-      -> SessionSubtype S2 T2
-      -> SessionSubtype (ReceiveT p S1 S2) (ReceiveT p T1 T2)
-  | SubSendDT : forall p τ S1 S2,
-      SessionSubtype S1 S2
-      -> SessionSubtype (SendDT p τ S1) (SendDT p τ S2)
-  | SubReceiveDT : forall p τ S1 S2,
-      SessionSubtype S1 S2
-      -> SessionSubtype (ReceiveDT p τ S1) (ReceiveDT p τ S2).
-  Infix "≤s" := SessionSubtype (at level 16).
-  Hint Constructors SessionSubtype : PiC.
-
-  CoFixpoint SubtypeRefl (T : SessionType) : T ≤s T :=
-    match T with
-    | EndType => SubEnd
-    | TypeVar n => SubVar n
-    | μ T' => SubμL _ _ (SubμR _ _ (SubtypeRefl _))
-    | EChoice p T1 => SubEChoice p T1 T1 (SubtypeRefl _)
-    | IChoice p T1 T2 => SubIChoice p T1 T2 T1 T2 (SubtypeRefl T1) (SubtypeRefl T2)
-    | SendT p T1 T2 => SubSend p T1 T2 T1 T2 (SubtypeRefl T1) (SubtypeRefl T2)
-    | ReceiveT p T1 T2 => SubReceive p T1 T2 T1 T2 (SubtypeRefl T1) (SubtypeRefl T2)
-    | SendDT p τ T' => SubSendDT p τ T' T' (SubtypeRefl T')
-    | ReceiveDT p τ T' => SubReceiveDT p τ T' T' (SubtypeRefl T')
-    end.
-
-  CoFixpoint SubtypeSym {S1 S2 : SessionType} (sub12 : S1 ≤s S2) : S2 ≤s S1 :=
-    match sub12 with
-    | SubEnd => SubEnd
-    | SubVar n => SubVar n
-    | SubμL T1 T2 pf => SubμR T2 T1 (SubtypeSym pf)
-    | SubμR T1 T2 pf => SubμL T2 T1 (SubtypeSym pf)
-    | SubEChoice p T1 T2 pf => SubEChoice p T2 T1 (SubtypeSym pf)
-    | SubIChoice p S1 S2 T1 T2 pf1 pf2 =>
-      SubIChoice p _ _ _ _ (SubtypeSym pf1)  (SubtypeSym pf2)
-    | SubSend p S1 S2 T1 T2 pf1 pf2 =>
-      SubSend p _ _ _ _ (SubtypeSym pf1) (SubtypeSym pf2)
-    | SubReceive p S1 S2 T1 T2 pf1 pf2 =>
-      SubReceive p _ _ _ _ (SubtypeSym pf1) (SubtypeSym pf2)
-    | SubSendDT p τ S1 S2 pf => SubSendDT p τ _ _ (SubtypeSym pf)
-    | SubReceiveDT p τ S1 S2 pf => SubReceiveDT p τ S2 S1 (SubtypeSym pf)
-    end.
-
-  Program CoFixpoint SubtypeSubst {S1 S2 : SessionType} (sub12 : S1 ≤s S2)
-          (σ : nat -> SessionType) : S1 [s| σ] ≤s S2 [s| σ] :=
-    match sub12 with
-    | SubEnd => SubEnd
-    | SubVar n => SubtypeRefl (σ n)
-    | SubμL T1 T2 pf => _
-    | SubμR T1 T2 pf => _
-    | SubEChoice p T1 T2 pf => SubEChoice p _ _ (SubtypeSubst pf σ)
-    | SubIChoice p S1 S2 T1 T2 pf1 pf2 =>
-      SubIChoice p _ _ _ _ (SubtypeSubst pf1 σ) (SubtypeSubst pf2 σ)
-    | SubSend p S1 S2 T1 T2 x x0 => _
-    | SubReceive p S1 S2 T1 T2 x x0 => _
-    | SubSendDT p τ S1 S2 x => _
-    | SubReceiveDT p τ S1 S2 x => _
-    end.
-  Next Obligation.
-  Admitted.
-  Next Obligation.
-  Admitted.
-  Next Obligation.
-    
-    
-
-  Program CoFixpoint SubtypeTrans {S1 S2 S3 : SessionType} (sub12 : S1 ≤s S2) (sub23 : S2 ≤s S3)
-    : S1 ≤s S3 :=
-    match sub12 with
-    | SubEnd => sub23
-    | SubVar n => sub23
-    | SubμL T1 T2 pf => SubμL T1 S3 (SubtypeTrans pf sub23)
-    | SubμR T1 T2 pf1 =>
-      match sub23 with
-      | SubEnd => _
-      | SubVar n => _
-      | SubμL T1 T2 pf2 => _
-      | SubμR T1 T2 x => _
-      | SubEChoice p T1 T2 x => _
-      | SubIChoice p S1 S2 T1 T2 x x0 => _
-      | SubSend p S1 S2 T1 T2 x x0 => _
-      | SubReceive p S1 S2 T1 T2 x x0 => _
-      | SubSendDT p τ S1 S2 x => _
-      | SubReceiveDT p τ S1 S2 x => _
+    Fixpoint GSTypeInd (T : GSType) : Q T :=
+      match T with
+      | Gμ T' => μCase T' (GSType'Ind T')
+      | GSTypeVar n => VarCase n
+      | GPlain T' => PlainCase T' (GSType'Ind T')
       end
-    | SubEChoice p T1 T2 x => _
-    | SubIChoice p T1 T2 T1' T2' x x0 => _
-    | SubSend p S1 S2 T1 T2 x x0 => _
-    | SubReceive p S1 S2 T1 T2 x x0 => _
-    | SubSendDT p τ S1 S2 x => _
-    | SubReceiveDT p τ S1 S2 x => _
-    end.
-  Next Obligation.
-    
-  Next Obligation.
-  
-  Theorem EndSubtype : forall T : SessionType, EndType ≤s T -> T = EndType.
-  Proof.
-    intro T; induction T; intro endsub; auto with PiC.
-    all: try (inversion endsub; fail).
-    inversion endsub.
-  
-  CoFixpoint SubtypeTrans {S1 S2 S3 : SessionType} (sub12 : S1 ≤s S2) (sub23 : S2 ≤s S3)
-    : S1 ≤ S3 :=
-    
-  
-  Lemma SubtypeRefl : forall S : SessionType, S ≤s S.
-  Proof.
-    intros S; induction S; auto with PiC.
-    apply SubμR. apply SubμL.
+    with GSType'Ind (T' : GSType') : P T' :=
+           match T' with
+           | GEndType => EndCase
+           | GSendType p τ T => SendCase p τ T (GSTypeInd T)
+           | GRecvType p τ T => RecvCase p τ T (GSTypeInd T)
+           | GEChoiceType p T => EChoiceCase p T (GSTypeInd T)
+           | GIChoiceType p T1 T2 => IChoiceCase p T1 T2 (GSTypeInd T1) (GSTypeInd T2)
+           end.
+  End GSTypeInd.
 
+  Fixpoint GSTypeRename (T : GSType) (ξ : nat -> nat) : GSType :=
+    match T with
+    | Gμ T' => Gμ (GSType'Rename T' (RenamingUp ξ))
+    | GSTypeVar n => GSTypeVar (ξ n)
+    | GPlain T' => GPlain (GSType'Rename T' ξ)
+    end
+  with GSType'Rename (T : GSType') (ξ : nat -> nat) : GSType' :=
+         match T with
+         | GEndType => GEndType
+         | GSendType p τ T => GSendType p τ (GSTypeRename T ξ)
+         | GRecvType p τ T => GRecvType p τ (GSTypeRename T ξ)
+         | GEChoiceType p T => GEChoiceType p (GSTypeRename T ξ)
+         | GIChoiceType p T1 T2 => GIChoiceType p (GSTypeRename T1 ξ) (GSTypeRename T2 ξ)
+         end.
+  Notation "T ⟨gst| ξ ⟩" := (GSTypeRename T ξ) (at level 15).
+  Notation "T ⟨gst'| ξ ⟩" := (GSType'Rename T ξ) (at level 15).
 
-  Instance sessionSubtypeRefl  : Reflexive SessionSubtype  := SubRefl.
-  Instance sessionSubtypeTrans : Transitive SessionSubtype := SubTrans.
-
-  Inductive PiCtxtRed : (Chan -> SessionType) -> (Chan -> SessionType) -> Prop :=
-    DataCommCtxtR : forall (Γ Δ : Chan -> SessionType) (s : nat) (p q : Role) (τ : ExprTyp)
-                      (S1 S2 : SessionType),
-      Γ (Session s p) = SendDT q τ S1
-      -> Γ (Session s q) = ReceiveDT p τ S2
-      -> Δ (Session s p) = S1
-      -> Δ (Session s q) = S2
-      -> (forall χ : Chan, (Session s p) <> χ -> (Session s q) <> χ -> Γ χ = Δ χ)
-      -> PiCtxtRed Γ Δ                         
-  | CommCtxtR : forall (Γ Δ : Chan -> SessionType) (s : nat) (p q  : Role)
-                  (S1 S2 T1 T2 : SessionType),
-      Γ (Session s p) = SendT q S1 S2
-      -> Γ (Session s q) = ReceiveT p T1 T2
-      -> S1 ≤s T1
-      -> Δ (Session s p) = S2
-      -> Δ (Session s q) = T2
-      -> (forall χ : Chan, (Session s p) <> χ -> (Session s q) <> χ -> Γ χ = Δ χ)
-      -> PiCtxtRed Γ Δ
-  | ChoiceCtxtR1 : forall (Γ Δ : Chan -> SessionType) (s : nat) (p q : Role)
-                     (S T1 T2 : SessionType),
-      Γ (Session s p) = EChoice q S
-      -> Γ (Session s q) = IChoice p T1 T2
-      -> Δ (Session s p) = S
-      -> Δ (Session s q) = T1
-      -> (forall χ : Chan, (Session s p) <> χ -> (Session s q) <> χ -> Γ χ = Δ χ)
-      -> PiCtxtRed Γ Δ
-  | ChoiceCtxtR2 : forall (Γ Δ : Chan -> SessionType) (s : nat) (p q : Role)
-                     (S T1 T2 : SessionType),
-      Γ (Session s p) = EChoice q S
-      -> Γ (Session s q) = IChoice p T1 T2
-      -> Δ (Session s p) = S
-      -> Δ (Session s q) = T2
-      -> (forall χ : Chan, (Session s p) <> χ -> (Session s q) <> χ -> Γ χ = Δ χ)
-      -> PiCtxtRed Γ Δ
-  | MuCtxtR : forall (Γ1 Γ2 Δ : Chan -> SessionType) (χ : Chan) (S1 : SessionType),
-      Γ1 χ = S1 [s| fun n => match n with
-                          | 0 => μ S1
-                          | S n' => TypeVar n'
-                          end]
-      -> Γ2 χ = μ S1
-      -> (forall χ2 : Chan, χ <> χ2 -> Γ1 χ2 = Γ2 χ2)
-      -> PiCtxtRed Γ1 Δ
-      -> PiCtxtRed Γ2 Δ.
-  Hint Constructors PiCtxtRed : PiC.
-
-  Inductive PiCtxtManyRed : (Chan -> SessionType) -> (Chan -> SessionType) -> Prop :=
-    PiCtxtManyZero : forall Γ : Chan -> SessionType, PiCtxtManyRed Γ Γ
-  | PiCtxtManySucc : forall Γ1 Γ2 Γ3 : Chan -> SessionType,
-      PiCtxtRed Γ1 Γ2 -> PiCtxtManyRed Γ2 Γ3 -> PiCtxtManyRed Γ1 Γ3.
-  Hint Constructors PiCtxtManyRed : PiC.
-  Lemma PiCtxtManyOne : forall Γ1 Γ2 : Chan -> SessionType,
-      PiCtxtRed Γ1 Γ2 -> PiCtxtManyRed Γ1 Γ2.
-  Proof.
-    intros Γ1 Γ2 red; eauto with PiC.
-  Qed.                                                            
-  
-  Definition EndCtxt : (Chan -> SessionType) -> Prop :=
-    fun Γ => forall χ, Γ χ ≤s EndType.
-
-  Definition SafetyCtxtProperty : ((Chan -> SessionType) -> Prop ) -> Prop :=
-    fun φ => forall Γ : Chan -> SessionType,
-        φ Γ ->
-        (forall (χ1 χ2 : Chan) (p q : Role)(S1 S2 T1 T2 : SessionType),
-            Γ χ1 = SendT p S1 S2
-            -> Γ χ2 = ReceiveT q T1 T2
-            -> S1 ≤s T1)
-        /\ (forall (χ : Chan) (S : SessionType),
-              Γ χ = μ S
-              -> φ (fun χ2 => if ChanEqDec χ χ2
-                         then S [s| fun k =>
-                                      match k with
-                                      | 0 => μ S
-                                      | S n' => TypeVar n'
-                                      end]
-                         else Γ χ2))
-        /\ (forall Δ, PiCtxtRed Γ Δ -> φ Δ).
-
-  Definition DFCtxt : (Chan -> SessionType) -> Prop :=
-    fun Γ : Chan -> SessionType => forall Δ : Chan -> SessionType,
-        PiCtxtManyRed Γ Δ ->
-        forall Δ', ~(PiCtxtRed Δ Δ') -> EndCtxt Δ'.
-
-  Definition LiveCtxt : (Chan -> SessionType) -> Prop :=
-    fun Γ => (forall (χ : Chan) (p : Role) (S1 S2 : SessionType),
-              Γ χ = SendT p S1 S2
-              -> exists (Γ' : Chan -> SessionType), Γ' χ = S2 /\ PiCtxtManyRed Γ Γ')
-          /\ (forall (χ : Chan) (p : Role) (S1 S2 : SessionType),
-                Γ χ = ReceiveT p S1 S2
-                -> exists (Γ' : Chan -> SessionType), Γ' χ = S2 /\ PiCtxtManyRed Γ Γ')
-          /\ (forall (χ : Chan) (p : Role) (S : SessionType),
-                Γ χ = EChoice p S
-                -> (exists (Γ' : Chan -> SessionType), Γ' χ = S /\ PiCtxtManyRed Γ Γ'))
-          /\ (forall (χ : Chan) (p : Role) (S1 S2 : SessionType),
-                Γ χ = IChoice p S1 S2
-                -> (exists (Γ' : Chan -> SessionType), Γ' χ = S1 /\ PiCtxtManyRed Γ Γ')
-                  /\ (exists (Γ' : Chan -> SessionType), Γ' χ = S2 /\ PiCtxtManyRed Γ Γ')).
-  Axiom LiveSafety : SafetyCtxtProperty LiveCtxt. (* From Lemma 5.9 in "Less is More" *)
-  Axiom LiveToDF : forall Γ : Chan -> SessionType, LiveCtxt Γ -> DFCtxt Γ. (* From Lemma 5.9 in "Less is More" *)
-  
-  Inductive PiCalc : Set :=
-    EndPi : PiCalc
-  | PiVar : nat -> PiCalc
-  | Par : PiCalc -> PiCalc -> PiCalc
-  | ν : PiCalc -> PiCalc
-  | Sel : Chan -> Role -> Coq.Init.Datatypes.bool -> PiCalc -> PiCalc
-  | Branch : Chan -> Role -> PiCalc -> PiCalc -> PiCalc
-  | Send : Chan -> Role -> Chan -> PiCalc -> PiCalc
-  | Receive : Chan -> Role -> PiCalc -> PiCalc
-  | Def : PiCalc -> PiCalc -> PiCalc
-  | SendD : Chan -> Role -> Expr -> PiCalc -> PiCalc
-  | ReceiveD : Chan -> Role -> PiCalc -> PiCalc
-  | IfThenElse : Expr -> PiCalc -> PiCalc -> PiCalc.
-  Notation "P ∥ Q" := (Par P Q) (at level 20).
-
-  Fixpoint PiCalcRename (P : PiCalc) (ξ : nat -> nat) : PiCalc :=
-    match P with
-    | EndPi => EndPi
-    | PiVar n => PiVar (ξ n)
-    | Par P Q => (PiCalcRename P ξ) ∥ (PiCalcRename Q ξ)
-    | ν P => ν (PiCalcRename P ξ)
-    | Sel χ p b P => Sel χ p b (PiCalcRename P ξ)
-    | Branch χ p P Q => Branch χ p (PiCalcRename P ξ) (PiCalcRename Q ξ)
-    | Send χ1 p χ2 P => Send χ1 p χ2 (PiCalcRename P ξ)
-    | Receive χ p P => Receive χ p (PiCalcRename P ξ)
-    | Def P Q => Def (PiCalcRename P (RenamingUp ξ)) (PiCalcRename Q (RenamingUp ξ))
-    | SendD χ p e P => SendD χ p e (PiCalcRename P ξ)
-    | ReceiveD χ p P => ReceiveD χ p (PiCalcRename P ξ)
-    | IfThenElse e P Q => IfThenElse e (PiCalcRename P ξ) (PiCalcRename Q ξ)
-    end.
-  Notation "P ⟨π| ξ ⟩" := (PiCalcRename P ξ) (at level 15).
-  Lemma PiCalcRenameExt : forall (P : PiCalc) (ξ1 ξ2 : nat -> nat),
-      (forall n, ξ1 n = ξ2 n) ->
-      P ⟨π| ξ1⟩ = P ⟨π| ξ2⟩.
-  Proof.
-    intros P; induction P; simpl; intros ξ1 ξ2 ext_eq; auto.
-    1,4,10: erewrite IHP1; eauto with PiC; erewrite IHP2; eauto.
-    1,2,3,4,6,7: erewrite IHP; eauto.
-    rewrite IHP1 with (ξ2 := RenamingUp ξ2); auto with PiC;
-      rewrite IHP2 with (ξ2 := RenamingUp ξ2); auto with PiC.
-  Qed.
-  
-  Fixpoint PiCalcRenameChan (P : PiCalc) (ξ : nat -> nat) : PiCalc :=
-    match P with
-    | EndPi => EndPi
-    | PiVar n => PiVar n
-    | P ∥ Q => (PiCalcRenameChan P ξ) ∥ (PiCalcRenameChan Q ξ)
-    | ν P => ν (PiCalcRenameChan P ξ)
-    | Sel χ p b P => Sel (ChanRename χ ξ) p b (PiCalcRenameChan P ξ)
-    | Branch χ p P Q => Branch (χ ⟨ch| ξ⟩) p (PiCalcRenameChan P ξ) (PiCalcRenameChan Q ξ)
-    | Send χ1 p χ2 P => Send (χ1 ⟨ch| ξ⟩) p (χ2 ⟨ch| ξ⟩) (PiCalcRenameChan P ξ)
-    | Receive χ p P => Receive (χ ⟨ch| ξ⟩) p (PiCalcRenameChan P (RenamingUp ξ))
-    | Def P Q => Def (PiCalcRenameChan P ξ) (PiCalcRenameChan Q ξ)
-    | SendD χ p e P => SendD (χ ⟨ch| ξ⟩) p e (PiCalcRenameChan P ξ)
-    | ReceiveD χ p P => ReceiveD (χ ⟨ch| ξ⟩) p (PiCalcRenameChan P ξ)
-    | IfThenElse e P Q => IfThenElse e (PiCalcRenameChan P ξ) (PiCalcRenameChan Q ξ)
-    end.
-  Notation "P ⟨πch| ξ ⟩" := (PiCalcRenameChan P ξ) (at level 15).
-
-  Lemma PiCalcRenameChanExt : forall (P : PiCalc) (ξ1 ξ2 : nat -> nat),
+  Lemma GSTypeRenameExt : forall (T : GSType) (ξ1 ξ2 : nat -> nat),
       (forall n, ξ1 n = ξ2 n)
-      -> P ⟨πch| ξ1⟩ = P ⟨πch| ξ2⟩.
+      -> T ⟨gst| ξ1⟩ = T ⟨gst| ξ2⟩.
   Proof.
-    intros P; induction P; intros ξ1 ξ2 ext_eq; simpl; auto.
-    3,4,5,6,8,9: assert (c ⟨ch| ξ1⟩ = c ⟨ch| ξ2⟩) as Hc by (apply ChanRenameExt; auto);
-      rewrite Hc; auto.
-    2,3,5,7,8: rewrite IHP with (ξ2 := ξ2); auto.
-    1,3,5,6: rewrite IHP1 with (ξ2 := ξ2); auto; rewrite IHP2 with (ξ2 := ξ2); auto.
-    - assert (c0 ⟨ch| ξ1⟩ = c0 ⟨ch| ξ2⟩) as Hc0 by (apply ChanRenameExt; auto);
-        rewrite Hc0; auto.
-    - rewrite IHP with (ξ2 := RenamingUp ξ2); auto.
-      apply RenamingUpExt; auto.
+    intro T;
+      induction T using GSTypeInd
+        with (P := fun T' =>
+                     forall ξ1 ξ2 : nat -> nat, (forall n, ξ1 n = ξ2 n) -> T' ⟨gst'|ξ1⟩ = T' ⟨gst'|ξ2⟩);
+      intros ξ1 ξ2 ext_eq; simpl; auto.
+    1,2,3,6: rewrite IHT with (ξ2 := ξ2); auto.
+    - rewrite IHT1 with (ξ2 := ξ2); [rewrite IHT2 with (ξ2 := ξ2)|]; auto.
+    - rewrite IHT with (ξ2 := RenamingUp ξ2); [reflexivity| apply RenamingUpExt; auto].
   Qed.
-  Hint Resolve PiCalcRenameChanExt : PiC.
-  Hint Rewrite PiCalcRenameChanExt : PiC.
+  Hint Resolve GSTypeRenameExt : PiC.
+  Hint Rewrite GSTypeRenameExt : PiC.
 
-  Lemma PiCalcIdRenameChan : forall P : PiCalc, P ⟨πch|IdRenaming⟩ = P.
-  Proof.
-    intro P; induction P; simpl; auto.
-    all: try (rewrite IHP; auto).
-    all: try (rewrite IHP1; rewrite IHP2; auto).
-    all: try (repeat rewrite ChanIdRenaming; auto).
-    assert (P ⟨πch| RenamingUp IdRenaming⟩ = P⟨πch| IdRenaming⟩)
-      by (apply PiCalcRenameChanExt; auto with PiC).
-    rewrite H; rewrite IHP; reflexivity.
-  Qed.
-
-  Fixpoint PiCalcSessionRename (P : PiCalc) (ξ : nat -> nat) : PiCalc :=
-    match P with
-    | EndPi => EndPi
-    | PiVar n => PiVar n
-    | Par P Q => (PiCalcSessionRename P ξ) ∥ (PiCalcSessionRename Q ξ)
-    | ν P => ν (PiCalcSessionRename P (RenamingUp ξ))
-    | Sel χ p b P => Sel (χ ⟨chs|ξ⟩) p b (PiCalcSessionRename P ξ)
-    | Branch χ p P Q =>
-      Branch (χ ⟨chs|ξ⟩) p (PiCalcSessionRename P ξ) (PiCalcSessionRename Q ξ)
-    | Send χ1 p χ2 P =>
-      Send (χ1 ⟨chs|ξ⟩) p (χ2 ⟨chs|ξ⟩) (PiCalcSessionRename P ξ)
-    | Receive χ p P =>
-      Receive (ChanSessionRename χ ξ) p (PiCalcSessionRename P ξ)
-    | Def P Q => Def (PiCalcSessionRename P ξ) (PiCalcSessionRename Q ξ)
-    | SendD χ p e P => SendD (χ ⟨chs| ξ⟩) p e (PiCalcSessionRename P ξ)
-    | ReceiveD χ p P => ReceiveD (χ ⟨chs| ξ⟩) p (PiCalcSessionRename P ξ)
-    | IfThenElse e P Q => IfThenElse e (PiCalcSessionRename P ξ) (PiCalcSessionRename Q ξ)
-    end.
-  Notation "P ⟨πs| ξ ⟩" := (PiCalcSessionRename P ξ) (at level 15).
-
-  Lemma PiCalcSessionRenameExt : forall (P : PiCalc) (ξ1 ξ2 : nat -> nat),
+  Lemma GSType'RenameExt : forall (T : GSType') (ξ1 ξ2 : nat -> nat),
       (forall n, ξ1 n = ξ2 n)
-      -> P ⟨πs| ξ1⟩ = P ⟨πs| ξ2⟩.
+      -> T ⟨gst'| ξ1⟩ = T ⟨gst'| ξ2⟩.
   Proof.
-    intro P; induction P; intros ξ1 ξ2 ext_eq; simpl; auto with PiC.
-    1,4,7,10: rewrite IHP1 with (ξ2 := ξ2); auto; rewrite IHP2 with (ξ2 := ξ2);
-      auto with PiC.
-    1,3,4,5,6,7: assert (c ⟨chs| ξ1⟩ = c⟨chs| ξ2⟩) as Hc
-        by (auto with PiC); rewrite Hc; auto.
-    1,2,3,4,5: rewrite IHP with (ξ2 := ξ2); auto.
-    - assert (c0 ⟨chs| ξ1⟩ = c0⟨chs| ξ2⟩) as Hc0
-        by (auto with PiC); rewrite Hc0; auto.
-    - rewrite IHP with (ξ2 := RenamingUp ξ2); auto with PiC.
+    intro T;
+      induction T using GSType'Ind
+        with (Q := fun T => forall ξ1 ξ2 : nat -> nat, (forall n, ξ1 n = ξ2 n) -> T ⟨gst|ξ1⟩ = T ⟨gst|ξ2⟩);
+      intros ξ1 ξ2 ext_eq; simpl; auto.
+    1,2,3,6: rewrite IHT with (ξ2 := ξ2); auto.
+    - rewrite IHT with (ξ2 := ξ2); [rewrite IHT0 with (ξ2 := ξ2)|]; auto.
+    - rewrite IHT with (ξ2 := RenamingUp ξ2); [reflexivity| apply RenamingUpExt; auto].
   Qed.
-  Hint Resolve PiCalcSessionRenameExt : PiC.
-  Hint Rewrite PiCalcSessionRenameExt : PiC.
 
-  Lemma PiCalcSessionIdRenaming : forall (P : PiCalc), P⟨πs| IdRenaming⟩ = P.
+  Lemma GSTypeRenameId : forall (T : GSType), T ⟨gst| IdRenaming⟩ = T.
   Proof.
-    intro P; induction P; simpl; auto with PiC.
-    1,4,7,10: rewrite IHP1; rewrite IHP2; auto.
-    1,3,4,5,6,7: repeat rewrite ChanIdSessionRenaming; auto.
-    1,2,3,4,5: rewrite IHP; auto.
-    rewrite PiCalcSessionRenameExt with (ξ2 := IdRenaming); auto with PiC.
-    rewrite IHP; reflexivity.
+    intro T; induction T using GSTypeInd
+               with (P := fun T' => T' ⟨gst'| IdRenaming⟩ = T'); simpl; auto.
+    1,2,3,6: rewrite IHT; reflexivity.
+    - rewrite IHT1; rewrite IHT2; reflexivity.
+    - rewrite GSType'RenameExt with (ξ2 := IdRenaming);
+        [rewrite IHT; reflexivity | exact IdRenamingUp].
   Qed.
-  Hint Resolve PiCalcSessionIdRenaming : PiC.
-  Hint Rewrite PiCalcSessionIdRenaming : PiC.
-
-  Fixpoint PiCalcExprRename (P : PiCalc) (ξ : nat -> nat) : PiCalc :=
-    match P with
-    | EndPi => EndPi
-    | PiVar n => PiVar n
-    | Par P Q => (PiCalcExprRename P ξ) ∥ (PiCalcExprRename Q ξ)
-    | ν P => ν (PiCalcExprRename P ξ)
-    | Sel χ p b P => Sel χ p b (PiCalcExprRename P ξ)
-    | Branch χ p P Q => Branch χ p (PiCalcExprRename P ξ) (PiCalcExprRename Q ξ)
-    | Send χ1 p χ2 P => Send χ1 p χ2 (PiCalcExprRename P ξ)
-    | Receive χ p P => Receive χ p (PiCalcExprRename P ξ)
-    | Def P Q => Def (PiCalcExprRename P ξ) (PiCalcExprRename Q ξ)
-    | SendD χ p e P => SendD χ p (e ⟨e|ξ⟩) (PiCalcExprRename P ξ)
-    | ReceiveD χ p P => ReceiveD χ p (PiCalcExprRename P (RenamingUp ξ))
-    | IfThenElse e P Q => IfThenElse (e ⟨e| ξ⟩) (PiCalcExprRename P ξ) (PiCalcExprRename Q ξ)
-    end.
-  Notation "P ⟨πe| ξ ⟩" := (PiCalcExprRename P ξ) (at level 15).
-
-  Lemma PiCalcExprRenameExt : forall (P : PiCalc) (ξ1 ξ2 : nat -> nat),
-      (forall n, ξ1 n = ξ2 n)
-      -> P ⟨πe| ξ1⟩ = P ⟨πe| ξ2⟩.
+  Lemma GSType'RenameId : forall (T : GSType'), T ⟨gst'| IdRenaming⟩ = T.
   Proof.
-    intro P; induction P; intros ξ1 ξ2 ext_eq; simpl; auto.
-    1,4,7,10: rewrite IHP1 with (ξ2 := ξ2); auto; rewrite IHP2 with (ξ2 := ξ2); auto.
-    2,3,4,5,6: rewrite IHP with (ξ2 := ξ2); auto.
-    1,2: rewrite ExprRenameExt with (ξ2 := ξ2); auto.
-    rewrite IHP with (ξ2 := RenamingUp ξ2); auto with PiC.
+    intro T; induction T using GSType'Ind
+               with (Q := fun T' => T' ⟨gst| IdRenaming⟩ = T'); simpl; auto.
+    1,2,3,6: rewrite IHT; reflexivity.
+    - rewrite IHT; rewrite IHT0; reflexivity.
+    - rewrite GSType'RenameExt with (ξ2 := IdRenaming);
+        [rewrite IHT; reflexivity | exact IdRenamingUp].
   Qed.
-  Hint Resolve PiCalcExprRenameExt : PiC.
-  Hint Rewrite PiCalcExprRenameExt : PiC.
 
-  Lemma PiCalcExprIdRenaming : forall (P : PiCalc),
-      P ⟨πe| IdRenaming⟩ = P.
-  Proof.
-    intro P; induction P; simpl; auto.
-    2,3,5,6,8: rewrite IHP; auto.
-    1,3,4,6: rewrite IHP1; rewrite IHP2; auto.
-    1,2: rewrite ExprIdRenamingSpec; reflexivity.
-    rewrite PiCalcExprRenameExt with (ξ2 := IdRenaming); [|apply IdRenamingUp].
-    rewrite IHP; auto.
-  Qed.
-  Hint Resolve PiCalcExprIdRenaming : PiC.
-  Hint Rewrite PiCalcExprIdRenaming : PiC.  
-  
-  Definition PiCalcSubstUp : (nat -> PiCalc) -> nat -> PiCalc :=
+  Definition GSTypeSubstUp : (nat -> GSType) -> nat -> GSType :=
     fun σ n => match n with
-            | 0 => PiVar n
-            | S n' => σ n' ⟨π| S⟩
+            | 0 => GSTypeVar 0
+            | S n' => σ n' ⟨gst| S⟩
             end.
-  Lemma PiCalcSubstUpExt : forall (σ1 σ2 : nat -> PiCalc),
+  
+  Fixpoint GSTypeSubst (T : GSType) (σ : nat -> GSType) :=
+    match T with
+    | Gμ T' => Gμ (GSType'Subst T' (GSTypeSubstUp σ))
+    | GSTypeVar n => σ n
+    | GPlain T' => GPlain (GSType'Subst T' σ)
+    end
+  with GSType'Subst (T' : GSType') (σ : nat -> GSType) :=
+    match T' with
+    | GEndType => GEndType
+    | GSendType p τ T => GSendType p τ (GSTypeSubst T σ)
+    | GRecvType p τ T => GRecvType p τ (GSTypeSubst T σ)
+    | GEChoiceType p T => GEChoiceType p (GSTypeSubst T σ)
+    | GIChoiceType p T1 T2 => GIChoiceType p (GSTypeSubst T1 σ) (GSTypeSubst T2 σ)
+    end.
+  Notation "P [gst| σ ]" := (GSTypeSubst P σ) (at level 15).
+  Notation "P [gst'| σ ]" := (GSType'Subst P σ) (at level 15).
+
+  Lemma GSTypeSubstExt : forall (T : GSType) (σ1 σ2 : nat -> GSType),
       (forall n, σ1 n = σ2 n)
-      -> forall n, PiCalcSubstUp σ1 n = PiCalcSubstUp σ2 n.
+      -> T [gst| σ1] = T [gst| σ2].
   Proof.
-    intros σ1 σ2 ext_eq n; unfold PiCalcSubstUp; destruct n; simpl; auto.
-    rewrite ext_eq; reflexivity.
+    intro T; induction T using GSTypeInd
+               with (P :=
+                       fun T' =>
+                         forall (σ1 σ2  : nat -> GSType),
+                           (forall n, σ1 n = σ2 n)
+                           -> T' [gst'| σ1] = T' [gst'| σ2]);
+    intros σ1 σ2 ext_eq; simpl; auto with PiC.
+    1,2,3,6: rewrite IHT with (σ2 := σ2); auto.
+    rewrite IHT1 with (σ2 := σ2); auto; rewrite IHT2 with (σ2 := σ2); auto.
+    rewrite IHT with (σ2 := GSTypeSubstUp σ2); [reflexivity|].
+    intro n; unfold GSTypeSubstUp; destruct n; simpl; [| rewrite ext_eq]; reflexivity.
+  Qed.    
+  Lemma GSType'SubstExt : forall (T : GSType') (σ1 σ2 : nat -> GSType),
+      (forall n, σ1 n = σ2 n)
+      -> T [gst'| σ1] = T [gst'| σ2].
+  Proof.
+    intro T; induction T using GSType'Ind
+               with (Q :=
+                       fun T' =>
+                         forall (σ1 σ2  : nat -> GSType),
+                           (forall n, σ1 n = σ2 n)
+                           -> T' [gst| σ1] = T' [gst| σ2]);
+    intros σ1 σ2 ext_eq; simpl; auto with PiC.
+    1,2,3,6: rewrite IHT with (σ2 := σ2); auto.
+    rewrite IHT with (σ2 := σ2); auto; rewrite IHT0 with (σ2 := σ2); auto.
+    rewrite IHT with (σ2 := GSTypeSubstUp σ2); [reflexivity|].
+    intro n; unfold GSTypeSubstUp; destruct n; simpl; [| rewrite ext_eq]; reflexivity.
   Qed.
-  Hint Resolve PiCalcSubstUpExt : PiC.
-  Hint Rewrite PiCalcSubstUpExt : PiC.
+
+  
+  
+  Inductive SType : Set :=
+    EndType : SType
+  | STypeVar : nat -> SType
+  | μ : SType -> SType
+  | SendType : Role -> ExprTyp -> SType -> SType
+  | RecvType : Role -> ExprTyp -> SType -> SType
+  | EChoiceType : Role -> SType -> SType
+  | IChoiceType : Role -> SType -> SType -> SType.
+  Hint Constructors SType : PiC.
+  
+  Fixpoint STypeRename (T : SType) (ξ : nat -> nat) : SType :=
+    match T with
+    | EndType => EndType
+    | STypeVar n => STypeVar (ξ n)
+    | μ T => μ (STypeRename T (RenamingUp ξ))
+    | SendType p τ T => SendType p τ (STypeRename T ξ)
+    | RecvType p τ T => RecvType p τ (STypeRename T ξ)
+    | EChoiceType p T => EChoiceType p (STypeRename T ξ)
+    | IChoiceType p T1 T2 => IChoiceType p (STypeRename T1 ξ) (STypeRename T2 ξ)
+    end.
+  Notation "T ⟨st| ξ ⟩" := (STypeRename T ξ) (at level 15).
+
+  Lemma STypeRenameExt : forall (T : SType) (ξ1 ξ2 : nat -> nat),
+      (forall n, ξ1 n = ξ2 n)
+      -> T ⟨st| ξ1⟩ = T ⟨st| ξ2⟩.
+  Proof.
+    intros T; induction T; intros ξ1 ξ2 ext_eq; simpl; auto with PiC.
+    2,3,4: rewrite IHT with (ξ2 := ξ2); auto.
+    - rewrite IHT with (ξ2 := RenamingUp ξ2);
+        [reflexivity| apply RenamingUpExt; exact ext_eq].
+    - rewrite IHT1 with (ξ2 := ξ2); auto; rewrite IHT2 with (ξ2 := ξ2); auto.
+  Qed.
+  Hint Resolve STypeRenameExt : PiC.
+  Hint Rewrite STypeRenameExt : PiC.
+
+  Lemma STypeRenameId : forall (T : SType), T ⟨st| IdRenaming⟩ = T.
+  Proof.
+    intro T; induction T; simpl; auto with PiC.
+    rewrite STypeRenameExt with (ξ2 := IdRenaming); [| exact IdRenamingUp].
+    1,2,3,4: rewrite IHT; reflexivity.
+    rewrite IHT1; rewrite IHT2; reflexivity.
+  Qed.
+  Hint Resolve STypeRenameId : PiC.
+  Hint Rewrite STypeRenameId : PiC.
+
+  Definition STypeSubstUp : (nat -> SType) -> nat -> SType :=
+    fun σ n => match n with
+            | 0 => STypeVar 0
+            | S n' => σ n' ⟨st| S ⟩
+            end.
+
+  Lemma STypeSubstUpExt : forall (σ1 σ2 : nat -> SType),
+      (forall n, σ1 n = σ2 n)
+      -> forall n, STypeSubstUp σ1 n = STypeSubstUp σ2 n.
+  Proof.
+    intros σ1 σ2 ext_eq n; unfold STypeSubstUp; destruct n; [|rewrite ext_eq]; reflexivity.
+  Qed.
+
+  Fixpoint STypeSubst (T : SType) (σ : nat -> SType) : SType :=
+    match T with
+    | EndType => EndType
+    | STypeVar n => σ n
+    | μ T => μ (STypeSubst T (STypeSubstUp σ))
+    | SendType p τ T => SendType p τ (STypeSubst T σ)
+    | RecvType p τ T => RecvType p τ (STypeSubst T σ)
+    | EChoiceType p T => EChoiceType p (STypeSubst T σ)
+    | IChoiceType p T1 T2 => IChoiceType p (STypeSubst T1 σ) (STypeSubst T2 σ)
+    end.
+  Notation "T [st| σ ]" := (STypeSubst T σ) (at level 15).
+
+  Lemma STypeSubstExt : forall (T : SType) (σ1 σ2 : nat -> SType),
+      (forall n, σ1 n = σ2 n)
+      -> T [st| σ1] = T [st| σ2].
+  Proof.
+    intro T; induction T; intros σ1 σ2 ext_eq; simpl; auto with PiC.
+    2,3,4: rewrite IHT with (σ2 := σ2); [reflexivity | exact ext_eq].
+    - rewrite IHT with (σ2 := STypeSubstUp σ2);
+        [reflexivity | apply STypeSubstUpExt; exact ext_eq].
+    - rewrite IHT1 with (σ2 := σ2); [| exact ext_eq];
+        rewrite IHT2 with (σ2 := σ2); [reflexivity| exact ext_eq].
+  Qed.
+  Hint Resolve STypeSubstExt : PiC.
+  Hint Rewrite STypeSubstExt : PiC.
+
+  Definition IdSTypeSubst : nat -> SType := STypeVar.
+  Lemma IdSTypeSubstUp : forall n, STypeSubstUp IdSTypeSubst n = IdSTypeSubst n.
+  Proof.
+    intro n; unfold STypeSubstUp; unfold IdSTypeSubst; destruct n; simpl; reflexivity.
+  Qed.
     
-  Fixpoint PiCalcSubst (P : PiCalc) (σ : nat -> PiCalc) : PiCalc :=
-    match P with
-    | EndPi => EndPi
-    | PiVar n => σ n
-    | Par P Q => (PiCalcSubst P σ) ∥ (PiCalcSubst Q σ)
-    | ν P => ν (PiCalcSubst P σ)
-    | Sel χ p b P => Sel χ p b (PiCalcSubst P σ)
-    | Branch χ p P Q => Branch χ p (PiCalcSubst P σ) (PiCalcSubst Q σ)
-    | Send χ1 p χ2 P => Send χ1 p χ2 (PiCalcSubst P σ)
-    | Receive χ p P => Receive χ p (PiCalcSubst P σ)
-    | Def P Q => Def (PiCalcSubst P (PiCalcSubstUp σ)) (PiCalcSubst Q (PiCalcSubstUp σ))
-    | SendD χ p e P => SendD χ p e (PiCalcSubst P σ)
-    | ReceiveD χ p P => ReceiveD χ p (PiCalcSubst P σ)
-    | IfThenElse e P Q => IfThenElse e (PiCalcSubst P σ) (PiCalcSubst Q σ)
-    end.
-  Notation "P [π| σ ]" := (PiCalcSubst P σ) (at level 15).
-
-  Lemma PiCalcSubstExt : forall (P : PiCalc) (σ1 σ2 : nat -> PiCalc),
-      (forall n, σ1 n = σ2 n)
-      -> P [π|σ1] = P [π|σ2].
+  Lemma STypeSubstId : forall (T : SType), T[st| IdSTypeSubst] = T.
   Proof.
-    intro P; induction P; intros σ1 σ2 ext_eq; simpl; auto with PiC.
-    1,4,10: erewrite IHP1; eauto; erewrite IHP2; eauto.
-    1,2,3,4,6,7: erewrite IHP; eauto.
-    rewrite IHP1 with (σ2 := PiCalcSubstUp σ2); [rewrite IHP2 with (σ2 := PiCalcSubstUp σ2)|];
-      auto with PiC.
+    intro T; induction T; simpl; auto with PiC.
+    rewrite STypeSubstExt with (σ2 := IdSTypeSubst); [| exact IdSTypeSubstUp].
+    1,2,3,4: rewrite IHT; reflexivity.
+    rewrite IHT1; rewrite IHT2; reflexivity.
   Qed.
-  Hint Resolve PiCalcSubstExt : PiC.
-  Hint Rewrite PiCalcSubstExt : PiC.
+  Hint Resolve STypeSubstId : PiC.
+  Hint Rewrite STypeSubstId : PiC.
 
-  Definition PiCalcIdSubst : nat -> PiCalc := PiVar.
-  Lemma PiCalcIdSubstUp : forall n, PiCalcSubstUp PiCalcIdSubst n = PiCalcIdSubst n.
+  Inductive Plain : SType -> Prop :=
+    EndPlain : Plain EndType
+  | SendPlain : forall p τ T, Plain (SendType p τ T)
+  | RecvPlain : forall p τ T, Plain (RecvType p τ T)
+  | EChoicePlain : forall p T, Plain (EChoiceType p T)
+  | IChoicePlain : forall p T1 T2, Plain (IChoiceType p T1 T2).
+
+  Lemma PlainRename : forall (T : SType) (ξ : nat -> nat),
+      Plain T -> Plain (T ⟨st| ξ⟩).
   Proof.
-    intros n; unfold PiCalcSubstUp; unfold PiCalcIdSubst; destruct n; simpl; reflexivity.
+    intro T; induction T; intros ξ nvT; simpl; auto; inversion nvT; constructor; auto.
   Qed.
-  Hint Resolve PiCalcIdSubstUp : PiC.
-  Hint Rewrite PiCalcIdSubstUp : PiC.
   
-  Lemma PiCalcIdSubstSpec : forall (P : PiCalc), P[π| PiCalcIdSubst] = P.
+  Lemma PlainSubst : forall (T : SType) (σ : nat -> SType),
+      Plain T -> Plain (T [st| σ]).
   Proof.
-    intro P; induction P; simpl; auto with PiC.
-    2,3,5,6,8,9: rewrite IHP; reflexivity.
-    1,2,4: rewrite IHP1; rewrite IHP2; reflexivity.
-    repeat rewrite PiCalcSubstExt
-      with (σ1 := PiCalcSubstUp PiCalcIdSubst) (σ2 := PiCalcIdSubst);
-      [rewrite IHP1; rewrite IHP2; reflexivity| |];
-      exact PiCalcIdSubstUp.
+    intro T; induction T; intros σ nvT; simpl; auto; inversion nvT; constructor; auto.
   Qed.
-  Hint Resolve PiCalcIdSubstSpec : PiC.
-  Hint Rewrite PiCalcIdSubstSpec : PiC.
 
-  Fixpoint PiCalcSubstChan (P : PiCalc) (σ : nat -> Chan) : PiCalc :=
-    match P with
-    | EndPi => EndPi
-    | PiVar n => PiVar n
-    | Par P Q => (PiCalcSubstChan P σ) ∥ (PiCalcSubstChan Q σ)
-    | ν P => ν (PiCalcSubstChan P σ)
-    | Sel χ p b P => Sel (χ [ch| σ]) p b (PiCalcSubstChan P σ)
-    | Branch χ p P Q => Branch (χ [ch| σ]) p (PiCalcSubstChan P σ) (PiCalcSubstChan Q σ)
-    | Send χ1 p χ2 P => Send (χ1 [ch| σ]) p (χ2 [ch| σ]) (PiCalcSubstChan P σ)
-    | Receive χ p P => Receive (χ [ch| σ]) p (PiCalcSubstChan P (ChanSubstUp σ))
-    | Def P Q => Def (PiCalcSubstChan P σ) (PiCalcSubstChan Q σ)
-    | SendD χ p e P => SendD (χ [ch| σ]) p e (PiCalcSubstChan P σ)
-    | ReceiveD χ p P => ReceiveD (χ [ch| σ]) p (PiCalcSubstChan P σ)
-    | IfThenElse e P Q => IfThenElse e (PiCalcSubstChan P σ) (PiCalcSubstChan Q σ)
-    end.
-  Notation "P [πch| σ ]" := (PiCalcSubstChan P σ) (at level 15).
+  Inductive GuardedType : SType -> Prop :=
+    EndGood : GuardedType EndType
+  | VarGood : forall n, GuardedType (STypeVar n)
+  | μGood : forall {T}, Plain T -> GuardedType T -> GuardedType (μ T)
+  | SendGood : forall (p : Role) (τ : ExprTyp) {T : SType},
+      GuardedType T -> GuardedType (SendType p τ T)
+  | RecvGood : forall (p : Role) (τ : ExprTyp) {T : SType},
+      GuardedType T -> GuardedType (RecvType p τ T)
+  | EChoiceGood : forall (p : Role) {T : SType}, GuardedType T -> GuardedType (EChoiceType p T)
+  | IChoiceGood : forall (p : Role) {T1 T2 : SType},
+      GuardedType T1 -> GuardedType T2 -> GuardedType (IChoiceType p T1 T2).
 
-  Lemma PiCalcSubstChanExt : forall (P : PiCalc) (σ1 σ2 : nat -> Chan),
-      (forall n, σ1 n = σ2 n)
-      -> P [πch| σ1] = P [πch| σ2].
+  Lemma GuardedTypeRename : forall (T : SType) (ξ : nat -> nat),
+      GuardedType T -> GuardedType (T ⟨st| ξ⟩).
   Proof.
-    intro P; induction P; intros σ1 σ2 ext_eq; simpl; auto with PiC.
-    2,3,5,8,9: rewrite IHP with (σ2 := σ2); auto with PiC.
-    1,6,8,9: rewrite IHP1 with (σ2 := σ2); auto; rewrite IHP2 with (σ2 := σ2);
-      auto with PiC.
-    all: assert (c[ch|σ1] = c[ch|σ2]) as Hc by (auto with PiC); rewrite Hc; auto.
-    - assert (c0[ch|σ1] = c0[ch|σ2]) as Hc0 by (auto with PiC); rewrite Hc0; auto.
-    - rewrite IHP with (σ2 := ChanSubstUp σ2); auto with PiC.
+    intro T; induction T; simpl; intros ξ gtT; auto; inversion gtT; constructor; auto.
+    apply PlainRename; auto.
   Qed.
-  Hint Resolve PiCalcSubstChanExt : PiC.
-  Hint Rewrite PiCalcSubstChanExt : PiC.
-
-  Lemma PiCalcSubstId : forall (P : PiCalc), P[πch| ChanIdSubst] = P.
-  Proof.
-    intro P; induction P; simpl; auto with PiC.
-    all: autorewrite with PiC.
-    2,3,5,8,9: rewrite IHP; reflexivity.
-    1,2,4,5: rewrite IHP1; rewrite IHP2; reflexivity.
-    assert (P [πch|ChanSubstUp ChanIdSubst] = P[πch|ChanIdSubst]) by (auto with PiC).
-    rewrite H; rewrite IHP; reflexivity.
-  Qed.
-  Hint Resolve PiCalcSubstId : PiC.
-  Hint Rewrite PiCalcSubstId : PiC.
-
-  Fixpoint PiCalcExprSubst (P : PiCalc) (σ : nat -> Expr) : PiCalc :=
-    match P with
-    | EndPi => EndPi
-    | PiVar n => PiVar n
-    | Par P Q => (PiCalcExprSubst P σ) ∥ (PiCalcExprSubst Q σ)
-    | ν P => ν (PiCalcExprSubst P σ)
-    | Sel χ p b P => Sel χ p b (PiCalcExprSubst P σ)
-    | Branch χ p P Q => Branch χ p (PiCalcExprSubst P σ) (PiCalcExprSubst Q σ)
-    | Send χ1 p χ2 P => Send χ1 p χ2 (PiCalcExprSubst P σ)
-    | Receive χ p P => Receive χ p (PiCalcExprSubst P σ)
-    | Def P Q => Def (PiCalcExprSubst P σ) (PiCalcExprSubst Q σ)
-    | SendD χ p e P => SendD χ p (e [e|σ]) (PiCalcExprSubst P σ)
-    | ReceiveD χ p P => ReceiveD χ p (PiCalcExprSubst P (ExprUpSubst σ))
-    | IfThenElse e P Q => IfThenElse (e [e|σ]) (PiCalcExprSubst P σ) (PiCalcExprSubst Q σ)
-    end.
-  Notation "P [πe| σ ]" := (PiCalcExprSubst P σ) (at level 15).
-
-  Theorem PiCalcExprSubstExt : forall (P : PiCalc) (σ1 σ2 : nat -> Expr),
-      (forall n, σ1 n = σ2 n)
-      -> P [πe| σ1] = P [πe| σ2].
-  Proof.
-    intros P; induction P; intros σ1 σ2 ext_eq; simpl; auto.
-    1,4,7,10: rewrite IHP1 with (σ2 := σ2); auto; rewrite IHP2 with (σ2 := σ2); auto.
-    2,3,4,5,6: rewrite IHP with (σ2 := σ2); auto.
-    1,2: rewrite ExprSubstExt with (σ2 := σ2); auto.
-    rewrite IHP with (σ2 := ExprUpSubst σ2); [reflexivity|].
-    intro n; unfold ExprUpSubst; destruct n; auto; rewrite ext_eq; reflexivity.
-  Qed.
-  Hint Resolve PiCalcExprSubstExt : PiC.
-  Hint Rewrite PiCalcExprSubstExt : PiC.
-
-  Theorem PiCaclExprSubstId : forall (P : PiCalc),
-      P [πe| ExprIdSubst] = P.
-  Proof.
-    intro P; induction P; simpl; auto.
-    8,10: rewrite ExprIdentitySubstSpec.
-    1,4,7,9: rewrite IHP1; rewrite IHP2; reflexivity.
-    1,2,3,4,5: rewrite IHP; reflexivity.
-    rewrite PiCalcExprSubstExt with (σ2 := ExprIdSubst).
-    rewrite IHP; reflexivity.
-    intro n; unfold ExprUpSubst; unfold ExprIdSubst; destruct n; simpl; auto.
-    apply ExprRenameVar.
-  Qed.
-  Hint Resolve PiCaclExprSubstId : PiC.
-  Hint Rewrite PiCaclExprSubstId : PiC.
-
-  Inductive PiEquiv' : PiCalc -> PiCalc -> Prop :=
-    SwapBranch : forall P Q, PiEquiv' (P ∥ Q) (Q ∥ P)
-  | ParAssoc : forall P Q R, PiEquiv' (P ∥ (Q ∥ R)) ((P ∥ Q) ∥ R)
-  | ParEnd : forall P, PiEquiv' (P ∥ EndPi) P
-  | NuEnd : PiEquiv' (ν EndPi) EndPi
-  | SwapNu : forall P, PiEquiv' (ν (ν P)) (ν (ν (P ⟨πs| fun n => match n with
-                                                        | 0 => 1
-                                                        | 1 => 0
-                                                        | m => m
-                                                         end⟩))).
-  Hint Constructors PiEquiv' : PiC.
-  Inductive PiEquiv : PiCalc -> PiCalc -> Prop :=
-    PiEquivRefl : forall P, PiEquiv P P
-  | LiftEquiv' : forall P Q, PiEquiv' P Q -> PiEquiv P Q
-  | PiEquivSym : forall P Q, PiEquiv P Q -> PiEquiv Q P
-  | PiEquivTrans : forall P Q R, PiEquiv P Q -> PiEquiv Q R -> PiEquiv P R.
-  Hint Constructors PiEquiv : PiC.
-
-  Inductive PiRedCtxt : Set :=
-    EmptyRedCtxt : PiRedCtxt
-  | ParCtxt : PiRedCtxt -> PiCalc -> PiRedCtxt
-  | NuCtxt : PiRedCtxt -> PiRedCtxt
-  | DefCtxt : PiCalc -> PiRedCtxt -> PiRedCtxt.
-
-  Fixpoint ApplyPiCtxt (CC : PiRedCtxt) (P : PiCalc) : PiCalc :=
-    match CC with
-    | EmptyRedCtxt => P
-    | ParCtxt CC' Q => (ApplyPiCtxt CC' P) ∥ Q
-    | NuCtxt CC' => ν (ApplyPiCtxt CC' P)
-    | DefCtxt Q CC' => Def Q (ApplyPiCtxt CC' P)
-    end.
-
-  Definition SendSubst (χ : Chan) : nat -> Chan := fun n => match n with
-                                                     | 0 => χ
-                                                     | S n' => ChanVar n'
-                                                     end.
-  Definition DefSubst (P : PiCalc) : nat -> PiCalc := fun n =>
-                                                      match n with
-                                                      | 0 => Def P (PiVar 0)
-                                                      | S n' => PiVar n'
-                                                      end.
-  Definition SendExprSubst (e : Expr) : nat -> Expr := fun n =>
-                                                     match n with
-                                                     | 0 => e
-                                                     | S n' => ExprVar n'
-                                                     end.
     
-  Inductive PiRed : PiCalc -> PiCalc -> Prop :=
-  | IfThenElseE : forall e1 e2 P Q,
-      ExprStep e1 e2
-      -> PiRed (IfThenElse e1 P Q) (IfThenElse e2 P Q)
-  | IfThenElseTrue : forall P Q,
-      PiRed (IfThenElse tt P Q) P
-  | IfThenElseFalse : forall P Q,
-      PiRed (IfThenElse ff P Q) Q
-  | RCommE : forall χ p e1 e2 P,
-      ExprStep e1 e2
-      -> PiRed (SendD χ p e1 P) (SendD χ p e2 P)
-  | RCommD : forall s p q v P Q,
-      ExprVal v ->
-      PiRed ((SendD (Session s p) q v P) ∥ (ReceiveD (Session s q) p Q))
-            (P ∥ (Q [πe|SendExprSubst v]))
-  | RComm : forall s p q χ P Q,
-      PiRed ((Send (Session s p) q χ P) ∥ (Receive (Session s q) p Q))
-            (P ∥ (Q [πch|SendSubst χ]))
-  | RChoice1 : forall s p q P Q1 Q2,
-      PiRed ((Sel (Session s p) q true P) ∥ (Branch (Session s q) p Q1 Q2))
-            (P ∥ Q1)
-  | RChoice2 : forall s p q P Q1 Q2,
-      PiRed ((Sel (Session s p) q false P) ∥ (Branch (Session s q) p Q1 Q2))
-            (P ∥ Q2)
-  | RDef : forall P Q, PiRed (Def P Q) (Q [π|DefSubst P])
-  | RCtxt : forall P Q,
-      PiRed P Q
-      -> forall CC : PiRedCtxt, PiRed (ApplyPiCtxt CC P) (ApplyPiCtxt CC Q)
-  | REq : forall P P' Q Q',
-      PiEquiv P P'
-      -> PiRed P' Q'
-      -> PiEquiv Q' Q
-      -> PiRed P Q.
-  Hint Constructors PiRed : PiC.
+  Lemma GuardedTypeSubst : forall (T : SType) (σ : nat -> SType),
+      GuardedType T -> (forall n, GuardedType (σ n)) -> GuardedType (T [st| σ]).
+  Proof.
+    intro T; induction T; simpl; intros σ gtT gtσ; inversion gtT; auto;
+      constructor; auto.
+    apply PlainSubst; auto.
+    apply IHT; auto. intro n; unfold STypeSubstUp; destruct n; [constructor|].
+    apply GuardedTypeRename; auto.
+  Qed.
 
-  Inductive PiRedMany : PiCalc -> PiCalc -> Prop :=
-    PiRedManyZero : forall P : PiCalc, PiRedMany P P
-  | PiRedManySucc : forall P Q R : PiCalc,
-      PiRed P Q
-      -> PiRedMany Q R
-      -> PiRedMany P R.
-  Hint Constructors PiRedMany : PiC.
+  Fixpoint FlattenGSType (T : GSType) : SType :=
+    match T with
+    | Gμ T' => μ (FlattenGSType' T')
+    | GSTypeVar n => STypeVar n
+    | GPlain T' => FlattenGSType' T'
+    end
+  with FlattenGSType' (T' : GSType') : SType :=
+         match T' with
+         | GEndType => EndType
+         | GSendType p τ T => SendType p τ (FlattenGSType T)
+         | GRecvType p τ T => RecvType p τ (FlattenGSType T)
+         | GEChoiceType p T => EChoiceType p (FlattenGSType T)
+         | GIChoiceType p T1 T2 => IChoiceType p (FlattenGSType T1) (FlattenGSType T2)
+         end.
 
-  Definition PiRedToMany : forall P Q, PiRed P Q -> PiRedMany P Q :=
-    fun P Q step => PiRedManySucc P Q Q step (PiRedManyZero Q).
-  Hint Resolve PiRedToMany : PiC.
+  Lemma FlattenGSTypeGuarded : forall (T : GSType), GuardedType (FlattenGSType T).
+  Proof.
+    intro T; induction T using GSTypeInd with (P := fun T' => GuardedType (FlattenGSType' T')
+                                                          /\ Plain (FlattenGSType' T'));
+    simpl; try split; try (constructor; auto; fail).
+    all: destruct IHT; auto; constructor; auto.
+  Qed.
 
-  Definition PiCalcDF : PiCalc -> Prop :=
-    fun P => forall Q, PiRedMany P Q -> (forall R, ~ PiRed Q R) -> PiEquiv Q EndPi.
-
-  Definition PiCalcLive : PiCalc -> Prop :=
-    fun P => forall (CC : PiRedCtxt) (Q : PiCalc),
-        PiRedMany P (ApplyPiCtxt CC Q)
-        -> (forall χ1 p χ2 Q',
-              Q = Send χ1 p χ2 Q'
-              -> exists CC' : PiRedCtxt, PiRedMany (ApplyPiCtxt CC Q) (ApplyPiCtxt CC' Q'))
-          /\ (forall χ p b Q',
-                Q = Sel χ p b Q'
-                -> exists CC' : PiRedCtxt, PiRedMany (ApplyPiCtxt CC Q) (ApplyPiCtxt CC' Q'))
-          /\ (forall χ p Q',
-                Q = Receive χ p Q'
-                -> exists CC' : PiRedCtxt, PiRedMany (ApplyPiCtxt CC Q) (ApplyPiCtxt CC' Q'))
-          /\ (forall χ p Q1 Q2,
-                Q = Branch χ p Q1 Q2
-                -> exists (CC' : PiRedCtxt) (Q' : PiCalc),
-                  (Q' = Q1 \/ Q' = Q2) 
-                  /\ PiRedMany (ApplyPiCtxt CC Q) (ApplyPiCtxt CC' Q')).
 
   
-  Definition ChannelTyping : (Chan -> SessionType) -> Chan -> SessionType -> Prop :=
-    fun Γ χ T => Γ χ ≤s T.
-  Notation "Γ ⊢ch χ ::: T" := (ChannelTyping Γ χ T) (at level 30).
+  Fixpoint TypeToGType (T : SType) : option GSType :=
+    match T with
+    | EndType => Some (GPlain (GEndType))
+    | STypeVar n => Some (GSTypeVar n)
+    | μ T' =>
+      match TypeToGType' T' with
+      | Some T'' => Some (Gμ T'')
+      | None => None
+      end
+    | SendType p τ T1 =>
+      match TypeToGType T1 with
+      | Some T2 => Some (GPlain (GSendType p τ T2))
+      | None => None
+      end
+    | RecvType p τ T1 =>
+      match TypeToGType T1 with
+      | Some T2 => Some (GPlain (GRecvType p τ T2))
+      | None => None
+      end
+    | EChoiceType p T1 =>
+      match TypeToGType T1 with
+      | Some T2 => Some (GPlain (GEChoiceType p T2))
+      | None => None
+      end
+    | IChoiceType p T11 T21 =>
+      match TypeToGType T11 with
+      | Some T12 =>
+        match TypeToGType T21 with
+        | Some T22 => Some (GPlain (GIChoiceType p T12 T22))
+        | None => None
+        end
+      | None => None
+      end
+    end
+  with TypeToGType' (T' : SType) : option GSType' :=
+         match T' with
+         | EndType => Some GEndType
+         | SendType p τ T1 =>
+           match TypeToGType T1 with
+           | Some T2 => Some (GSendType p τ T2)
+           | None => None
+           end
+         | RecvType p τ T1 =>
+           match TypeToGType T1 with
+           | Some T2 => Some (GRecvType p τ T2)
+           | None => None
+           end
+         | EChoiceType p T1 =>
+           match TypeToGType T1 with
+           | Some T2 => Some (GEChoiceType p T2)
+           | None => None
+           end
+         | IChoiceType p T11 T21 =>
+           match TypeToGType T11 with
+           | Some T12 => match TypeToGType T21 with
+                        | Some T22 => Some (GIChoiceType p T12 T22)
+                        | None => None
+                        end
+           | None => None
+           end
+         | _ => None
+         end.
 
-  (* TODO: Add in stuff about sending and receiving data *)
+  Lemma GuardedPlainTypeToGTypeMaster : forall (T : SType),
+      GuardedType T -> (exists GT, TypeToGType T = Some GT)
+                      /\ (Plain T -> exists GT', TypeToGType' T = Some GT').
+  Proof.
+    intro T; induction T; intros gT.
+    all: split;[|intro pT]; simpl; try (eexists; eauto; fail).
+    all: try (inversion pT; fail).
+    all: inversion gT.
+    all: repeat match goal with
+                | [H: ?P, IH : ?P -> ?Q |- _] => specialize (IH H)
+                | [H : ?P /\ ?Q |- _] => destruct H
+                | [H : exists x, TypeToGType ?T = Some x |- _] =>
+                  let GT := fresh "GT" in
+                  let HGT := fresh "HGT" in 
+                  destruct H as [GT HGT]
+                | [H : exists x, TypeToGType' ?T = Some x |- _] =>
+                  let GT := fresh "GT'" in
+                  let HGT := fresh "HGT'" in 
+                  destruct H as [GT HGT]
+                end.
+    all: try (rewrite HGT; eexists; eauto; fail).
+    rewrite HGT'; eexists; eauto.
+    all: rewrite HGT; rewrite HGT0; eexists; eauto.
+  Qed.        
   
-  Reserved Notation "Θ ;; Γ ⋅ Δ ⊢st P" (at level 30).
-  Inductive ProcessTyping : nat -> (Chan -> SessionType) -> (nat -> ExprTyp) -> PiCalc -> Prop :=
-  | EndST : forall Θ Γ Δ, EndCtxt Γ -> Θ ;; Γ ⋅ Δ ⊢st EndPi
-  | VarST : forall Θ Γ Δ n, n < Θ -> EndCtxt Γ -> Θ ;; Γ ⋅ Δ ⊢st PiVar n
-  | DefST : forall Θ Γ Δ P Q,
-      (S Θ) ;; Γ ⋅ Δ ⊢st P
-      -> (S Θ) ;; Γ ⋅ Δ ⊢st Q
-      -> Θ ;; Γ ⋅ Δ ⊢st Def P Q
-  | SendST : forall Θ Γ Δ p χ1 χ2 P S1 S2,
-      χ1 <> χ2 (* To guarantee linearity *)
-      -> Γ ⊢ch χ1 ::: SendT p S1 S2
-      -> Γ ⊢ch χ2 ::: S1
-      -> Θ ;; (fun χ' => if ChanEqDec χ1 χ'
-                    then S2
-                    else if ChanEqDec χ2 χ'
-                         then EndType (* Again, to guarantee linearity *)
-                         else Γ χ') ⋅ Δ ⊢st P
-      -> Θ ;; Γ ⋅ Δ ⊢st (Send χ1 p χ2 P)
-  | ReceiveST : forall Θ Γ Δ p χ P S1 S2,
-      Γ ⊢ch χ ::: ReceiveT p S1 S2
-      -> Θ ;; (fun χ' => match χ' with
-                    | ChanVar n => match n with
-                                  | 0 => S1
-                                  | S n' => if ChanEqDec (ChanVar n') χ
-                                           then S2
-                                           else Γ (ChanVar n')
-                                  end
-                    | Session _ _ => if ChanEqDec χ' χ
-                                    then S2
-                                    else Γ χ
-                    end) ⋅ Δ ⊢st P
-      -> Θ ;; Γ ⋅ Δ ⊢st (Receive χ p P)
-  | SendDST : forall Θ Γ Δ χ p e τ P S,
-      Δ ⊢e e ::: τ
-      -> Γ ⊢ch χ ::: SendDT p τ S
-      -> Θ ;; (fun χ' => if ChanEqDec χ χ'
-                    then S
-                    else Γ χ') ⋅ Δ ⊢st P
-      -> Θ ;; Γ ⋅ Δ ⊢st SendD χ p e P
-  | ReceiveDST : forall Θ Γ Δ χ p τ P S,
-      Γ ⊢ch χ ::: ReceiveDT p τ S
-      -> Θ ;; (fun χ' => if ChanEqDec χ χ'
-                   then S
-                   else Γ χ') ⋅ (fun n => match n with
-                                       | 0 => τ
-                                       | S n' => Δ n'
-                                       end) ⊢st P
-      -> Θ ;; Γ ⋅ Δ ⊢st ReceiveD χ p P 
-  | BranchST : forall Θ Γ Δ χ p P1 P2 S1 S2,
-      Γ ⊢ch χ ::: IChoice p S1 S2
-      -> Θ ;; (fun χ' => if ChanEqDec χ χ'
-                    then S1
-                    else Γ χ') ⋅ Δ ⊢st P1
-      -> Θ ;; (fun χ' => if ChanEqDec χ χ'
-                    then S2
-                    else Γ χ') ⋅ Δ ⊢st P2
-      -> Θ ;; Γ ⋅ Δ ⊢st Branch χ p P1 P2
-  | SelST : forall Θ Γ Δ χ p b P S,
-      Γ ⊢ch χ ::: EChoice p S
-      -> Θ ;; (fun χ' => if ChanEqDec χ χ'
-                    then S
-                    else Γ χ') ⋅ Δ ⊢st P
-      -> Θ ;; Γ ⋅ Δ ⊢st Sel χ p b P
-  | NuST : forall Θ Γ1 Γ2 Δ P,
-      (forall χ : Chan, (exists p : Role, χ = Session 0 p)
-                   \/ Γ2 χ ≤s EndType)
-      -> LiveCtxt Γ2
-      -> Θ ;; (fun χ => match χ with
-                   | ChanVar _ => Γ1 χ
-                   | Session n p => match n with
-                                   | 0 => Γ2 χ
-                                   | S n' => Γ1 (Session n' p)
-                                   end
-                   end) ⋅ Δ ⊢st P
-      -> Θ ;; Γ1 ⋅ Δ ⊢st ν P
-  | ParST : forall Θ Γ Γ1 Γ2 Δ P Q,
-      Θ ;; Γ1 ⋅ Δ ⊢st P
-      -> Θ ;; Γ2 ⋅ Δ ⊢st Q
-      -> (forall χ, Γ1 χ = EndType \/ Γ2 χ = EndType) (* Linearity *)
-      -> (forall χ, if SessionTypeEqDec (Γ1 χ) EndType then Γ χ = Γ2 χ else Γ χ = Γ1 χ)
-      -> Θ ;; Γ ⋅ Δ ⊢st P ∥ Q
-  | IfST : forall Θ Γ Δ e P Q,
-      Δ ⊢e e ::: bool
-      -> Θ ;; Γ ⋅ Δ ⊢st P
-      -> Θ ;; Γ ⋅ Δ ⊢st Q
-      -> Θ ;; Γ ⋅ Δ ⊢st IfThenElse e P Q          
-  where "Θ ;; Γ ⋅ Δ ⊢st P" := (ProcessTyping Θ Γ Δ P).
+  Lemma GuardedTypeToGType : forall (T : SType),
+      GuardedType T -> exists GT, TypeToGType T = Some GT.
+  Proof.
+    apply GuardedPlainTypeToGTypeMaster.
+  Qed.
 
-  Inductive WithClosedExpressions
+  Lemma GuardedPlainTypeToGType : forall (T : SType),
+      GuardedType T -> Plain T -> exists GT', TypeToGType' T = Some GT'.
+  Proof.
+    apply GuardedPlainTypeToGTypeMaster.
+  Qed.
 
-  (* An immediate consequence of 4.16 from "Less is More" *)
-  Axiom SubjRed : forall (Θ : nat) (Γ : Chan -> SessionType) (Δ : nat -> ExprTyp) (P : PiCalc),
-      Θ ;; Γ ⋅ Δ ⊢st P -> LiveCtxt Γ -> forall P' : PiCalc, PiRed P P' -> Θ ;; Γ ⋅ Δ ⊢st P'.
+  Lemma STypeThroughGTypeIdMaster : forall (T : SType),
+      (forall GT : GSType, TypeToGType T = Some GT -> FlattenGSType GT = T)
+      /\ (forall GT' : GSType', TypeToGType' T = Some GT' -> FlattenGSType' GT' = T).
+  Proof.
+    intro T; induction T; split.
+    1,3,5,7,9,11,13: intros GT eq.
+    8,9,10,11,12,13,14: intros GT' eq.
+    all: simpl in *; try (inversion eq; simpl; auto; fail).
+    all: try (destruct IHT; destruct (TypeToGType T); inversion eq).
+    destruct (TypeToGType' T) eqn:e; inversion eq.
+    simpl. rewrite (H0 g0 eq_refl). reflexivity.
+    destruct (TypeToGType' T) eqn:e; inversion eq.
+    simpl. rewrite (H0 g eq_refl). reflexivity.
+    all: simpl.
+    all: try (match goal with
+              | [H : (forall g, Some ?g' = Some g -> FlattenGSType g = ?T) |- context[(FlattenGSType ?g')] ]
+                => rewrite (H g' eq_refl)
+              end; reflexivity).
+    all: destruct (TypeToGType T1) eqn:e1; [|inversion eq].
+    all: destruct (TypeToGType T2) eqn:e2; inversion eq; simpl in *.
+    all: destruct IHT1; destruct IHT2.
+    - rewrite (H g eq_refl); rewrite (H2 g0 eq_refl); reflexivity.
+    - rewrite (H g eq_refl); rewrite (H2 g0 eq_refl); reflexivity.
+  Qed.
+  Lemma STypeThroughGTypeId : forall (T : SType) (GT : GSType),
+      TypeToGType T = Some GT -> FlattenGSType GT = T.
+  Proof.
+    apply STypeThroughGTypeIdMaster.
+  Qed.
+  Lemma STypeThroughGType'Id : forall (T : SType) (GT : GSType'),
+      TypeToGType' T = Some GT -> FlattenGSType' GT = T.
+  Proof.
+    apply STypeThroughGTypeIdMaster.
+  Qed.
 
-  (* From Theorem 5.15 of "Less is More" *)
-  Axiom TypingDF : forall (Θ : nat) (Γ : Chan -> SessionType) (Δ : nat -> ExprTyp) (P : PiCalc),
-      LiveCtxt Γ -> Θ ;; Γ ⋅ Δ ⊢st P -> PiCalcDF P.
+  Lemma TypeToGType'ImpliesTypeToGType : forall (T : SType) (GT' :GSType'),
+      TypeToGType' T = Some GT' -> exists GT, TypeToGType T = Some GT.
+  Proof.
+    intro T; induction T; intros GT' HGT'; simpl in *; try (eexists; eauto; fail).
+    all: try (destruct (TypeToGType T));
+      repeat match goal with
+             | [ H : None = Some _ |- _ ] => inversion H
+             end; try (eexists; eauto; fail).
+    destruct (TypeToGType T1); destruct (TypeToGType T2); try (inversion HGT'; fail).
+    eexists; eauto.
+  Qed.
+  
+  Lemma GTypeThroughSType : forall GT : GSType, TypeToGType (FlattenGSType GT) = Some GT.
+  Proof.
+    intro GT; induction GT using GSTypeInd
+                with (P := fun GT' =>
+                             (TypeToGType' (FlattenGSType' GT') = Some GT')
+                             /\ (TypeToGType (FlattenGSType' GT') = Some (GPlain GT')));
+    simpl; auto.
+    all: try (rewrite IHGT); auto.
+    - rewrite IHGT1; rewrite IHGT2; auto.
+    - destruct IHGT. rewrite H. reflexivity.
+    - destruct IHGT. exact H0.
+  Qed.
 
-End MPST.
+  Lemma GType'ThroughSTypeMaster : forall (GT' : GSType'),
+      TypeToGType' (FlattenGSType' GT') = Some GT'
+      /\ TypeToGType (FlattenGSType' GT') = Some (GPlain GT').
+  Proof.
+    intro GT'; induction GT' using GSType'Ind
+                 with (Q := fun GT => TypeToGType (FlattenGSType GT) = Some GT);
+    simpl; auto.
+    all: try (rewrite IHGT'); auto.
+    - rewrite IHGT'0; auto.
+    - destruct IHGT'. rewrite H. reflexivity.
+    - destruct IHGT'. exact H0.
+  Qed.
+
+  Lemma GType'ThroughSType : forall (GT' : GSType'),
+      TypeToGType' (FlattenGSType' GT') = Some GT'.
+  Proof.
+    apply GType'ThroughSTypeMaster.
+  Qed.
+
+  Lemma GTypeThroughSType' :  forall (GT' : GSType'),
+      TypeToGType (FlattenGSType' GT') = Some (GPlain GT').
+  Proof.
+    apply GType'ThroughSTypeMaster.
+  Qed.
+
+  Lemma LiftTypeToGType' : forall (T : SType) (GT' : GSType'),
+      TypeToGType' T = Some GT' -> TypeToGType T = Some (GPlain GT').
+  Proof.
+    intro T; induction T; simpl; intros GT' eq; try (inversion eq; reflexivity; fail).
+    all: try (destruct (TypeToGType T); inversion eq; reflexivity).
+    destruct (TypeToGType T1); [|inversion eq];
+      destruct (TypeToGType T2); inversion eq; reflexivity.
+  Qed.                                                 
+
+  Lemma TypeToGTypeRenameMaster : forall (T : SType)(ξ : nat -> nat),
+      (forall GT : GSType,
+          TypeToGType T = Some GT
+          -> TypeToGType (T ⟨st| ξ⟩) = Some (GT ⟨gst| ξ⟩))
+      /\ (forall GT' : GSType',
+            TypeToGType' T = Some GT'
+            -> TypeToGType' (T ⟨st| ξ⟩) = Some (GT' ⟨gst'| ξ⟩)).
+  Proof.
+    intro T; induction T; intro ξ.
+    all: split; [intro GT | intro GT']; intro eq; simpl in *; auto;
+      try (inversion eq; simpl; auto; fail).
+    all: try (specialize (IHT ξ); destruct IHT as [IHT IHT'];
+              destruct (TypeToGType T) as [GT2|]; inversion eq;
+              rewrite IHT with (GT := GT2); simpl; reflexivity).
+    - destruct (IHT (RenamingUp ξ)) as [IHTξ IHT'ξ].
+      destruct (TypeToGType' T) as [GT'|]; [|inversion eq].
+      rewrite IHT'ξ with (GT'0 := GT'); [| reflexivity].
+      inversion eq. simpl. reflexivity.
+    - specialize (IHT1 ξ); destruct IHT1 as [IHT1 IHT1'].
+      specialize (IHT2 ξ); destruct IHT2 as [IHT2 IHT2'].
+      destruct (TypeToGType T1) as [GT1 |]; [|inversion eq];
+        destruct (TypeToGType T2) as [GT2 |]; inversion eq.
+      rewrite IHT1 with (GT := GT1); [|reflexivity].
+      rewrite IHT2 with (GT := GT2); reflexivity.
+    - specialize (IHT1 ξ); destruct IHT1 as [IHT1 IHT1'].
+      specialize (IHT2 ξ); destruct IHT2 as [IHT2 IHT2'].
+      destruct (TypeToGType T1) as [GT1 |]; [|inversion eq];
+        destruct (TypeToGType T2) as [GT2 |]; inversion eq.
+      rewrite IHT1 with (GT := GT1); [|reflexivity].
+      rewrite IHT2 with (GT := GT2); reflexivity.
+  Qed.
+  Lemma TypeToGTypeRename : forall (T : SType)(ξ : nat -> nat) (GT : GSType),
+      TypeToGType T = Some GT
+      -> TypeToGType (T ⟨st| ξ⟩) = Some (GT ⟨gst| ξ⟩).
+  Proof.
+    apply TypeToGTypeRenameMaster.
+  Qed.
+  Lemma TypeToGType'Rename : forall (T : SType) (ξ : nat -> nat) (GT' : GSType'),
+      TypeToGType' T = Some GT'
+      -> TypeToGType' (T ⟨st| ξ⟩) = Some (GT' ⟨gst'| ξ⟩).
+  Proof.
+    apply TypeToGTypeRenameMaster.
+  Qed.
       
+  Lemma TypeToGTypeSubstMaster : forall (T : SType)(σ : nat -> SType) (gσ : nat -> GSType),
+      (forall n, TypeToGType (σ n) = Some (gσ n))
+      -> (forall GT : GSType, TypeToGType T = Some GT
+         -> TypeToGType (T [st| σ]) = Some (GT [gst| gσ]))
+      /\ (forall GT' : GSType', TypeToGType' T = Some GT'
+         -> TypeToGType' (T [st| σ]) = Some (GT' [gst'| gσ])).
+  Proof.
+    intro T; induction T; intros σ gσ ext_eq.
+    all: split; [intros GT eq | intros GT' eq].
+    all: simpl in *; try (inversion eq; simpl; auto; fail).
+    all: try (specialize (IHT σ gσ ext_eq); destruct IHT as [IHT IHT'];
+              destruct (TypeToGType T) as [GT1 |]; inversion eq;
+              rewrite IHT with (GT := GT1); simpl; reflexivity).
+    2,3: specialize (IHT1 σ gσ ext_eq); destruct IHT1 as [IHT1 IHT1'];
+      specialize (IHT2 σ gσ ext_eq); destruct IHT2 as [IHT2 IHT2'];
+        destruct (TypeToGType T1) as [GT1 |]; [|inversion eq];
+          destruct (TypeToGType T2) as [GT2|]; inversion eq;
+            rewrite (IHT1 GT1); [|reflexivity]; rewrite (IHT2 GT2); simpl; reflexivity.
+    specialize IHT with (σ := STypeSubstUp σ) (gσ := GSTypeSubstUp gσ).
+    destruct IHT as [IHT IHT'].
+    intro n; destruct n; unfold STypeSubstUp; unfold GSTypeSubstUp; auto.
+    rewrite TypeToGTypeRename with (GT := gσ n); [reflexivity | apply ext_eq].
+    destruct (TypeToGType' T) as [GT' |]; inversion eq.
+    rewrite IHT' with (GT'0 := GT'); simpl; reflexivity.
+  Qed.
+
+  Lemma TypeToGTypeSubst : forall (T : SType)(σ : nat -> SType) (gσ : nat -> GSType) (GT : GSType),
+      (forall n, TypeToGType (σ n) = Some (gσ n))
+      -> TypeToGType T = Some GT
+      -> TypeToGType (T [st| σ]) = Some (GT [gst| gσ]).
+  Proof.
+    intros T σ gσ GT H H0.
+    apply TypeToGTypeSubstMaster; auto.
+  Qed.
+                                                      
+  Lemma TypeToGType'Subst : forall (T : SType)(σ : nat -> SType) (gσ : nat -> GSType) (GT' : GSType'),
+      (forall n, TypeToGType (σ n) = Some (gσ n))
+      -> TypeToGType' T = Some GT'
+      -> TypeToGType' (T [st| σ]) = Some (GT' [gst'| gσ]).
+  Proof.
+    intros T σ gσ GT' H H0.
+    apply TypeToGTypeSubstMaster; auto.
+  Qed.
+  
+  Definition σμ (T : SType) : nat -> SType :=
+    fun n => match n with
+          | 0 => μ T
+          | S n' => STypeVar n
+          end.
+            
+  Reserved Infix "≡st" (at level 16).
+  CoInductive STypeEquiv : SType -> SType -> Prop :=
+  | EndEquiv : EndType ≡st EndType
+  | VarEquiv : forall n, STypeVar n ≡st STypeVar n
+  | SendEquiv : forall (p : Role) (τ : ExprTyp) {T1 T2 : SType},
+      T1 ≡st T2 -> (SendType p τ T1) ≡st (SendType p τ T2)
+  | RecvEquiv : forall (p : Role) (τ : ExprTyp) {T1 T2 : SType},
+      T1 ≡st T2 -> (RecvType p τ T1) ≡st (RecvType p τ T2)
+  | EChoiceEquiv : forall (p : Role) {T1 T2 : SType},
+      T1 ≡st T2 -> (EChoiceType p T1) ≡st (EChoiceType p T2)
+  | IChoiceEquiv : forall (p : Role) {S1 S2 T1 T2 : SType},
+      S1 ≡st S2 -> T1 ≡st T2 -> (IChoiceType p S1 T1) ≡st (IChoiceType p S2 T2)
+  | μEquivL : forall {S T : SType}, (S [st| σμ S]) ≡st T -> (μ S) ≡st T
+  | μEquivR : forall {S T : SType}, S ≡st (T [st| σμ T]) -> S ≡st (μ T)
+  where "T1 ≡st T2" := (STypeEquiv T1 T2).
+
+  CoFixpoint STypeEquivRefl (T : SType) : T ≡st T :=
+    match T with
+    | EndType => EndEquiv
+    | STypeVar n => VarEquiv n
+    | μ T => μEquivL (μEquivR (STypeEquivRefl _))
+    | SendType p τ T => SendEquiv p τ (STypeEquivRefl T)
+    | RecvType p τ T => RecvEquiv p τ (STypeEquivRefl T)
+    | EChoiceType p T => EChoiceEquiv p (STypeEquivRefl T)
+    | IChoiceType p T1 T2 => IChoiceEquiv p (STypeEquivRefl T1) (STypeEquivRefl T2)
+    end.
+
+  CoFixpoint STypeEquivSym {T1 T2 : SType} (equiv12 : T1 ≡st T2) : T2 ≡st T1 :=
+    match equiv12 with
+    | EndEquiv => EndEquiv
+    | VarEquiv n => VarEquiv n
+    | SendEquiv p τ pf => SendEquiv p τ (STypeEquivSym pf)
+    | RecvEquiv p τ pf => RecvEquiv p τ (STypeEquivSym pf)
+    | EChoiceEquiv p pf => EChoiceEquiv p (STypeEquivSym pf)
+    | IChoiceEquiv p pf1 pf2 => IChoiceEquiv p (STypeEquivSym pf1) (STypeEquivSym pf2)
+    | μEquivL pf => μEquivR (STypeEquivSym pf)
+    | μEquivR pf => μEquivL (STypeEquivSym pf)
+    end.
+
+  Definition gσμ (T : GSType') : nat -> GSType :=
+    fun n => match n with
+          | 0 => Gμ T
+          | S n' => GSTypeVar n
+          end.
+
+  Reserved Infix "≡gst" (at level 16).
+  Reserved Infix "≡gst'" (at level 16).
+  CoInductive GSTypeEquiv : GSType -> GSType -> Prop :=
+  | GVarEquiv : forall n, GSTypeVar n ≡gst GSTypeVar n
+  | GμEquivL : forall {T1 : GSType'} {T2 : GSType},
+      (GPlain (T1 [gst'| gσμ T1])) ≡gst T2 -> (Gμ T1) ≡gst T2
+  | GμEquivR : forall {T1 : GSType} {T2 : GSType'},
+      T1 ≡gst GPlain (T2 [gst'| gσμ T2]) -> T1 ≡gst (Gμ T2)
+  | GPlainEquiv : forall {T1 T2 : GSType'},
+      T1 ≡gst' T2 -> GPlain T1 ≡gst GPlain T2
+  where "T1 ≡gst T2" := (GSTypeEquiv T1 T2)
+  with GSType'Equiv : GSType' -> GSType' -> Prop :=
+  | GEndEquiv : GEndType ≡gst' GEndType
+  | GSendEquiv : forall (p : Role) (τ : ExprTyp) {T1 T2 : GSType},
+      T1 ≡gst T2 -> (GSendType p τ T1) ≡gst' (GSendType p τ T2)
+  | GRecvEquiv : forall (p : Role) (τ : ExprTyp) {T1 T2 : GSType},
+      T1 ≡gst T2 -> (GRecvType p τ T1) ≡gst' (GRecvType p τ T2)
+  | GEChoiceEquiv : forall (p : Role) {T1 T2 : GSType},
+      T1 ≡gst T2 -> (GEChoiceType p T1) ≡gst' (GEChoiceType p T2)
+  | GIChoiceEquiv : forall (p : Role) {S1 S2 T1 T2 : GSType},
+      S1 ≡gst S2 -> T1 ≡gst T2 -> (GIChoiceType p S1 T1) ≡gst' (GIChoiceType p S2 T2)
+  where "T1 ≡gst' T2" := (GSType'Equiv T1 T2).
+
+  Lemma SigmaMuGuarded : forall (T1 : SType),
+      GuardedType T1 -> Plain T1 -> forall n, GuardedType (σμ T1 n).
+  Proof.
+    intros T1 GT1 PT1 n; unfold σμ; destruct n; [constructor; auto| constructor].
+  Qed.
+
+  Ltac GuardedTypeEquiv1Tac :=
+    repeat match goal with
+           | [ |- ?a = ?a ] => reflexivity
+           | [ H : TypeToGType _ = Some _ |- _ ] => simpl in H
+           | [ H : match (TypeToGType ?T) with
+                   | Some _ => _
+                   | None => _
+                   end = Some _ |- _] => destruct (TypeToGType T)
+           | [ H: None = Some _ |- _] => inversion H
+           | [ H : Some ?a = Some ?b |- _] =>
+             match goal with
+             | [_ : a = b |- _ ] => fail 1
+             |  _ => inversion H;
+                    assert (a = b) by (inversion H; auto)
+             end
+           end.
+
+  Obligation Tactic := program_simpl; GuardedTypeEquiv1Tac.
+
+  Program CoFixpoint GuardedTypeEquiv1 (T1 T2 : SType) (GT1 GT2 : GSType)
+          (eq1 : TypeToGType T1 = Some GT1) (eq2 : TypeToGType T2 = Some GT2)
+          (equiv : T1 ≡st T2) : GT1 ≡gst GT2 :=
+  match equiv with
+  | EndEquiv => GPlainEquiv (GEndEquiv)
+  | VarEquiv n => GVarEquiv n
+  | SendEquiv p τ equiv' =>
+    match GT1 with
+    | Gμ x => _
+    | GSTypeVar x => _
+    | GPlain GT1' =>
+      match GT1' with
+      | GEndType => _
+      | GSendType _ _ GT1'' =>
+        match GT2 with
+        | Gμ x => _
+        | GSTypeVar x => _
+        | GPlain GT2' =>
+          match GT2' with
+          | GEndType => _
+          | GSendType _ _ GT2'' =>
+            GPlainEquiv (GSendEquiv p τ (GuardedTypeEquiv1 _ _ GT1'' GT2'' _ _ equiv'))
+          | GRecvType x x0 x1 => _
+          | GEChoiceType x x0 => _
+          | GIChoiceType x x0 x1 => _
+          end
+        end
+      | GRecvType x x0 x1 => _
+      | GEChoiceType x x0 => _
+      | GIChoiceType x x0 x1 => _
+      end
+    end
+  | RecvEquiv p τ equiv' =>
+    match GT1 with
+    | Gμ x => _
+    | GSTypeVar x => _
+    | GPlain GT1' =>
+      match GT1' with
+      | GEndType => _
+      | GSendType x x0 x1 => _
+      | GRecvType _ _ GT1'' =>
+        match GT2 with
+        | Gμ x => _
+        | GSTypeVar x => _
+        | GPlain GT2' =>
+          match GT2' with
+          | GEndType => _
+          | GSendType x x0 x1 => _
+          | GRecvType _ _ GT2'' =>
+            GPlainEquiv (GRecvEquiv p τ (GuardedTypeEquiv1 _ _ GT1'' GT2'' _ _ equiv'))
+          | GEChoiceType x x0 => _
+          | GIChoiceType x x0 x1 => _
+          end
+        end
+      | GEChoiceType x x0 => _
+      | GIChoiceType x x0 x1 => _
+      end
+    end
+  | EChoiceEquiv p equiv' =>
+    match GT1 with
+    | Gμ x => _
+    | GSTypeVar x => _
+    | GPlain GT1' =>
+      match GT1' with
+      | GEndType => _
+      | GSendType x x0 x1 => _
+      | GRecvType x x0 x1 => _
+      | GEChoiceType _ GT1'' =>
+        match GT2 with
+        | Gμ x => _
+        | GSTypeVar x => _
+        | GPlain GT2' =>
+          match GT2' with
+          | GEndType => _
+          | GSendType x x0 x1 => _
+          | GRecvType x x0 x1 => _
+          | GEChoiceType _ GT2'' =>
+            GPlainEquiv (GEChoiceEquiv p (GuardedTypeEquiv1 _ _ GT1'' GT2'' _ _ equiv'))
+          | GIChoiceType x x0 x1 => _
+          end
+        end
+      | GIChoiceType x x0 x1 => _
+      end
+    end
+  | IChoiceEquiv p equiv'1 equiv'2 =>
+    match GT1 with
+    | Gμ x => _
+    | GSTypeVar x => _
+    | GPlain GT1' =>
+      match GT1' with
+      | GEndType => _
+      | GSendType x x0 x1 => _
+      | GRecvType x x0 x1 => _
+      | GEChoiceType x x0 => _
+      | GIChoiceType _ GT11 GT12 =>
+        match GT2 with
+        | Gμ x => _
+        | GSTypeVar x => _
+        | GPlain GT2' =>
+          match GT2' with
+          | GEndType => _
+          | GSendType x x0 x1 => _
+          | GRecvType x x0 x1 => _
+          | GEChoiceType x x0 => _
+          | GIChoiceType _ GT21 GT22 =>
+            GPlainEquiv (GIChoiceEquiv p (GuardedTypeEquiv1 _ _ GT11 GT21 _ _ equiv'1)
+                                       (GuardedTypeEquiv1 _ _ GT12 GT22 _ _ equiv'2))
+          end
+        end
+      end
+    end
+  | @μEquivL T1' _ equiv' =>
+    match (TypeToGType' T1') with
+    | Some T1'' => @GμEquivL T1'' _ (GuardedTypeEquiv1 _ _ _ _ _ _ equiv')
+    | None => _
+    end
+  | @μEquivR _ T2' equiv' =>
+    match (TypeToGType' T2') with
+    | Some T2'' =>  @GμEquivR _ T2'' (GuardedTypeEquiv1 _ _ _ _ _ _ equiv')
+    | None => _
+    end
+  end.
+  Next Obligation.
+    rewrite <- H0; rewrite <- H1; rewrite <- H4; rewrite <- H5; reflexivity.
+  Defined.
+  Next Obligation.
+    rewrite <- H0; rewrite <- H1; rewrite <- H4; rewrite <- H5; reflexivity.
+  Defined.
+  Next Obligation.
+    rewrite <- H0; rewrite <- H3; reflexivity.
+  Defined.
+  Next Obligation.
+    rewrite <- H0. rewrite <- H4. reflexivity.
+  Defined.
+  Next Obligation.
+    simpl in eq1. destruct (TypeToGType' T1') as [GT1'|] eqn:e; inversion eq1.
+    inversion Heq_anonymous.
+    rewrite TypeToGTypeSubst with (gσ := gσμ GT1') (GT := GPlain GT1').
+    simpl. reflexivity.
+    intro n; unfold σμ; unfold gσμ; destruct n; auto.
+    simpl. rewrite e. reflexivity.
+    apply LiftTypeToGType'; auto.
+  Defined.
+  Next Obligation.
+    simpl in eq1. destruct (TypeToGType' T1') as [GT1'|] eqn:e; inversion eq1.
+    inversion Heq_anonymous. rewrite <- H1. reflexivity.
+  Defined.
+  Next Obligation.
+    simpl in eq1. destruct (TypeToGType' T1'); [inversion Heq_anonymous | inversion eq1].
+  Defined.
+  Next Obligation.
+    destruct (TypeToGType' T2') as [GT2'|] eqn:e; inversion eq2.
+    inversion Heq_anonymous.
+    rewrite TypeToGTypeSubst with (gσ := gσμ GT2') (GT := GPlain GT2').
+    simpl; reflexivity.
+    intro n; unfold σμ; unfold gσμ; destruct n; auto.
+    simpl. rewrite e. reflexivity.
+    apply LiftTypeToGType'; auto.
+  Defined.
+  Next Obligation.
+    destruct (TypeToGType' T2'); inversion eq2.
+    inversion Heq_anonymous. reflexivity.
+  Defined.
+  Next Obligation.
+    destruct (TypeToGType' T2'); [inversion Heq_anonymous | inversion eq2].
+  Defined.
+
+  Program CoFixpoint GuardedTypeEquiv2 (T1 T2 : SType) (GT1 GT2 : GSType)
+          (eq1 : TypeToGType T1 = Some GT1) (eq2 : TypeToGType T2 = Some GT2)
+          (equiv : GT1 ≡gst GT2) : T1 ≡st T2 :=
+    match equiv with
+    | GVarEquiv n => VarEquiv n
+    | @GμEquivL GT1' _ equiv' => μEquivL (GuardedTypeEquiv2 _ _ (GPlain (GT1' [gst'| gσμ GT1'])) _ _ _ equiv')
+    | GμEquivR x => _
+    | GPlainEquiv equiv' => GuardedTypeEquiv2' _ _ _ _ _ _ equiv'
+    end
+  with GuardedTypeEquiv2' (T1 T2 : SType) (GT1' GT2' : GSType')
+          (eq1 : TypeToGType' T1 = Some GT1') (eq2 : TypeToGType' T2 = Some GT2')
+          (equiv : GT1' ≡gst' GT2') : T1 ≡st T2 :=
+         _.
+  Next Obligation.
+    destruct T1; simpl in eq1; inversion eq1. reflexivity.
+    all: try (destruct (TypeToGType' T1); inversion eq1; fail).
+    all: try (destruct (TypeToGType T1); inversion eq1; fail).
+    destruct (TypeToGType T1_1); [|inversion eq1];
+      destruct (TypeToGType T1_2); inversion eq1.
+  Defined.
+  Next Obligation.
+    destruct T2; simpl in eq2; inversion eq2. reflexivity.
+    all: try (destruct (TypeToGType' T2); inversion eq2; fail).
+    all: try (destruct (TypeToGType T2); inversion eq2; fail).
+    destruct (TypeToGType T2_1); [|inversion eq2];
+      destruct (TypeToGType T2_2); inversion eq2.
+  Defined.
+  Next Obligation.
+    unfold GuardedTypeEquiv2_obligation_3; simpl.
+    unfold eq_rec_r. simpl.
+    rewrite TypeToGTypeSubst with (gσ := gσμ GT1') (GT := GPlain GT1'); simpl.
+    reflexivity.
+    intro n; unfold σμ; unfold gσμ; destruct n; auto. simpl.
+                                         
+  (* Lemma SigmaMuConnection : forall (T1 : SType) (G : GuardedType T1) (P : Plain T1),  *)
+  (*     ReflectGuardedType (T1 [st| σμ T1]) *)
+  (*                        (GuardedTypeSubst T1 (σμ T1) G (SigmaMuGuarded T1 G P)) *)
+  (*     = (GSTypeSubst (ReflectGuardedType T1 G) (gσμ (ReflectGuardedPlainType T1 G P))). *)
+  (* Proof. *)
+  (*   intro T1; induction T1; intros G P; try (inversion G; inversion P; fail); auto. *)
+  (*   simpl. fold ReflectGuardedType. *)
+  (* Admitted. *)
+                                          
+  Program CoFixpoint GuardedTypeEquiv1 (T1 T2 : SType)
+          (G1 : GuardedType T1) (G2 : GuardedType T2)
+          (equiv : T1 ≡st T2)
+    : (ReflectGuardedType T1 G1) ≡gst (ReflectGuardedType T2 G2)
+    := match equiv with
+      | EndEquiv => GPlainEquiv GEndEquiv
+      | VarEquiv n => GVarEquiv n
+      | @SendEquiv p τ T1 T2 equiv' =>
+        GPlainEquiv (GuardedPlainTypeEquiv1 _ _ _ _
+                                            (SendPlain _ _ T1)
+                                            (SendPlain _ _ T2)
+                                            equiv)
+      | @RecvEquiv p τ T1 T2 equiv' =>
+        GPlainEquiv (GuardedPlainTypeEquiv1 _ _ G1 G2
+                                            (RecvPlain _ _ T1)
+                                            (RecvPlain _ _ T2)
+                                            equiv)
+      | @EChoiceEquiv p T1 T2 equiv' =>
+        GPlainEquiv (GuardedPlainTypeEquiv1 _ _ G1 G2
+                                            (EChoicePlain _ T1)
+                                            (EChoicePlain _ T2)
+                                            equiv)
+      | @IChoiceEquiv p S1 S2 T1 T2 equiv'1 equiv'2 =>
+        GPlainEquiv (GuardedPlainTypeEquiv1 _ _ G1 G2
+                                            (IChoicePlain _ S1 T1)
+                                            (IChoicePlain _ S2 T2)
+                                            equiv)
+      | @μEquivL T1' _ equiv' =>
+        @GμEquivL
+            (ReflectGuardedPlainType T1' _ _)
+            (ReflectGuardedType T2 _)
+            (GuardedTypeEquiv1 _ _ _ _  equiv')
+      | @μEquivR _ T2' equiv' =>
+        @GμEquivR
+          (ReflectGuardedType T1 _)
+          (ReflectGuardedPlainType T2' _ _)
+          (GuardedTypeEquiv1 _ _ _ _ equiv')
+      end
+  with GuardedPlainTypeEquiv1 (T1 T2 : SType)
+                             (G1 : GuardedType T1) (G2 : GuardedType T2)
+                             (P1 : Plain T1) (P2 : Plain T2)
+                             (equiv : T1 ≡st T2)
+       : (ReflectGuardedPlainType T1 G1 P1) ≡gst' (ReflectGuardedPlainType T2 G2 P2)
+       := match equiv with
+         | EndEquiv => GEndEquiv
+         | VarEquiv n => _
+         | SendEquiv p τ equiv' => GSendEquiv p τ (GuardedTypeEquiv1 _ _ _ _ equiv')
+         | RecvEquiv p τ equiv' => GRecvEquiv p τ (GuardedTypeEquiv1 _ _ _ _ equiv')
+         | EChoiceEquiv p equiv' => GEChoiceEquiv p (GuardedTypeEquiv1 _ _ _ _ equiv')
+         | IChoiceEquiv p equiv'1 equiv'2 =>
+           GIChoiceEquiv p (GuardedTypeEquiv1 _ _ _ _ equiv'1)
+                         (GuardedTypeEquiv1 _ _ _ _ equiv'2)
+                                                          
+         | μEquivL equiv' => _
+         | μEquivR equiv' => _
+         end.
+  Next Obligation.
+    inversion P1.
+  Defined.
+  Next Obligation.
+    inversion G1; auto.
+  Defined.
+  Next Obligation.
+    inversion G2; auto.
+  Defined.
+  Next Obligation.
+    inversion G1; auto.
+  Defined.
+  Next Obligation.
+    inversion G2; auto.
+  Defined.
+  Next Obligation.
+    inversion G1; auto.
+  Defined.
+  Next Obligation.
+    inversion G2; auto.
+  Defined.
+  Next Obligation.
+    inversion G1; auto.
+  Defined.
+  Next Obligation.
+    inversion G2; auto.
+  Defined.
+  Next Obligation.
+    inversion G1; auto.
+  Defined.
+  Next Obligation.
+    inversion G2; auto.
+  Defined.
+  Next Obligation.
+    inversion P1.
+  Defined.
+  Next Obligation.
+    inversion P2.
+  Defined.
+  Next Obligation.
+    inversion G1; auto.
+  Defined.
+  Next Obligation.
+    inversion G1; auto.
+  Defined.
+  Next Obligation.
+    apply GuardedTypeSubst. inversion G1; auto.
+    unfold σμ. intro n; destruct n; constructor; auto;
+    inversion G1; auto.
+  Defined.
+  Next Obligation.
+  Admitted.
+  Next Obligation.
+    inversion G2; auto.
+  Defined.
+  Next Obligation.
+    inversion G2; auto.
+  Defined.
+  Next Obligation.
+    apply GuardedTypeSubst. inversion G2; auto.
+    unfold σμ; intro n; destruct n; constructor; auto; inversion G2; auto.
+  Defined.
+  Next Obligation.
+  Admitted.
+
+  Program CoFixpoint GSTypeEquivTrans {T1 T2 T3 : GSType}
+          (equiv12 : T1 ≡gst T2) (equiv23 : T2 ≡gst T3) : T1 ≡gst T3 :=
+    match equiv12 with
+    | GVarEquiv n => equiv23
+    | GμEquivL equiv' =>
+      match equiv' with
+      | GVarEquiv n => GμEquivL equiv23
+      | GμEquivL equiv'' => _
+      | GμEquivR equiv'' =>
+        match equiv'' with
+        | GVarEquiv n => _
+        | GμEquivL x => _
+        | GμEquivR x => _
+        | GPlainEquiv equiv'''' =>
+          match equiv23 with
+          | GVarEquiv n => _
+          | GμEquivL equiv''' =>
+            match equiv''' with
+            | GVarEquiv n => _
+            | GμEquivL x => _
+            | GμEquivR equiv'''' =>
+              match equiv'''' with
+              | GVarEquiv n => _
+              | GμEquivL  x => _
+              | GμEquivR  x => _
+              | GPlainEquiv equiv''''' => GμEquivL (GμEquivR (GSTypeEquivTrans equiv''
+                                                                              _))
+              end
+            | GPlainEquiv x => GμEquivL (GSTypeEquivTrans _ equiv''')
+            end
+          | GμEquivR equiv''' => GμEquivR (GSTypeEquivTrans _ equiv''')
+          | GPlainEquiv x => _
+          end
+        end
+      | GPlainEquiv equiv'' => GμEquivL (GSTypeEquivTrans _ equiv23)
+      end
+    | GμEquivR equiv12' =>
+      match equiv23 with
+      | GVarEquiv n => _
+      | GμEquivL equiv23' =>
+        match equiv12' with
+        | GVarEquiv n => _
+        | GμEquivL equiv12'' => GμEquivL (GSTypeEquivTrans equiv12'' equiv23')
+        | GμEquivR x => _
+        | GPlainEquiv equiv12'' =>
+          match equiv23' with
+          | GVarEquiv n => _
+          | GμEquivL x => _
+          | GμEquivR equiv23'' => GμEquivR (GSTypeEquivTrans _ equiv23'')
+          | GPlainEquiv equiv23'' => GPlainEquiv (GSType'EquivTrans _ equiv23'')
+          end
+        end
+      | GμEquivR equiv23' =>
+        match equiv23' with
+        | GVarEquiv n => _
+        | GμEquivL equiv23'' => GμEquivR (GSTypeEquivTrans _ equiv23'')
+        | GμEquivR x => _
+        | GPlainEquiv x => _
+        end
+      | GPlainEquiv x => _
+      end
+    | GPlainEquiv equiv12' =>
+      match equiv23 with
+      | GVarEquiv n => _
+      | GμEquivL x => _
+      | GμEquivR equiv23' => GμEquivR (GSTypeEquivTrans equiv12 equiv23')
+      | GPlainEquiv equiv23' => GPlainEquiv (GSType'EquivTrans equiv12' equiv23')
+      end
+    end
+  with GSType'EquivTrans {T1 T2 T3 : GSType'}
+                         (equiv12 : T1 ≡gst' T2) (equiv23 : T2 ≡gst' T3) : T1 ≡gst' T3 :=
+         match equiv12 with
+         | GEndEquiv => _
+         | GSendEquiv p τ equiv12' =>
+           match equiv23 with
+           | GEndEquiv => _
+           | GSendEquiv _ _ equiv23' => GSendEquiv p τ (GSTypeEquivTrans equiv12' equiv23')
+           | GRecvEquiv p τ x => _
+           | GEChoiceEquiv p x => _
+           | GIChoiceEquiv p x x0 => _
+           end
+         | GRecvEquiv p τ equiv12' =>
+           match equiv23 with
+           | GEndEquiv => _
+           | GSendEquiv p τ x => _
+           | GRecvEquiv _ _ equiv23' => GRecvEquiv p τ (GSTypeEquivTrans equiv12' equiv23')
+           | GEChoiceEquiv p x => _
+           | GIChoiceEquiv p x x0 => _
+           end
+         | GEChoiceEquiv p equiv12' =>
+           match equiv23 with
+           | GEndEquiv => _
+           | GSendEquiv p τ x => _
+           | GRecvEquiv p τ  x => _
+           | GEChoiceEquiv p equiv23' => GEChoiceEquiv p (GSTypeEquivTrans equiv12' equiv23')
+           | GIChoiceEquiv p x x0 => _
+           end
+         | GIChoiceEquiv p equiv12' equiv12'' =>
+           match equiv23 with
+           | GEndEquiv => _
+           | GSendEquiv p τ x => _
+           | GRecvEquiv p τ x => _
+           | GEChoiceEquiv p x => _
+           | GIChoiceEquiv p equiv23' equiv23'' =>
+             GIChoiceEquiv p (GSTypeEquivTrans equiv12' equiv23')
+                           (GSTypeEquivTrans equiv12'' equiv23'')
+           end
+         end.
+    
+  Program CoFixpoint STypeEquivAllμX : forall T : SType, T ≡st μ (STypeVar 0) :=
+    fun T => μEquivR (STypeEquivAllμX T).
+
+  Theorem STypeEquivTransToTrivial :
+    (forall {T1 T2 T3 : SType}, T1 ≡st T2 -> T2 ≡st T3 -> T1 ≡st T3) ->
+  forall {T1 T2 : SType}, T1 ≡st T2.
+  Proof.
+    intros stetrans T1 T2. apply stetrans with (T2 := μ (STypeVar 0)). 
+    apply STypeEquivAllμX. apply STypeEquivSym. apply STypeEquivAllμX.
+  Qed.
+
+  Theorem STypeEquivNotTrivial : ~ (EndType ≡st STypeVar 0).
+  Proof.
+    intro H. inversion H.
+  Qed.
+
+  Theorem STypeEquivNotTransitive : ~(forall T1 T2 T3 : SType, T1 ≡st T2 -> T2 ≡st T3 -> T1 ≡st T3).
+  Proof.
+    intro stetrans. apply STypeEquivNotTrivial. apply stetrans with (T2 := μ (STypeVar 0)).
+    apply STypeEquivAllμX. apply STypeEquivSym. apply STypeEquivAllμX.
+  Qed.
+
+  Inductive CtxtStep : (Role -> SType) -> (Role -> SType) -> Prop :=
+  | CtxtCommStep : forall Γ Γ' p q τ S T,
+      Γ p = SendType q τ S
+      -> Γ q  = RecvType p τ T
+      -> Γ' p = S
+      -> Γ' q = T
+      -> (forall (r : Role), r <> p -> r <> q -> Γ r = Γ' r)
+      -> CtxtStep Γ Γ'
+  | CtxtChoiceStep1 : forall Γ Γ' p q S T1 T2,
+      Γ p = EChoiceType q S
+      -> Γ q = IChoiceType p T1 T2
+      -> Γ' p = S
+      -> Γ' q = T1
+      -> (forall (r : Role), r <> p -> r <> q -> Γ r = Γ' r)
+      -> CtxtStep Γ Γ'
+  | CtxtChoiceStep2 : forall Γ Γ' p q S T1 T2,
+      Γ p = EChoiceType q S
+      -> Γ q = IChoiceType p T1 T2
+      -> Γ' p = S
+      -> Γ' q = T2
+      -> (forall (r : Role), r <> p -> r <> q -> Γ r = Γ' r)
+      -> CtxtStep Γ Γ'
+  | CtxtμStep : forall Γ Γ' p S,
+      Γ p = μ S
+      -> Γ' p = S [st| σμ S]
+      -> (forall (r : Role), r <> p -> Γ r = Γ' r)
+      -> CtxtStep Γ Γ'.
+
+  Lemma CtxtStepExt : forall Γ1 Γ2 Γ1' Γ2',
+      (forall r : Role, Γ1 r = Γ1' r)
+      -> (forall r : Role, Γ2 r = Γ2' r)
+      -> CtxtStep Γ1 Γ2
+      -> CtxtStep Γ1' Γ2'.
+  Proof.
+    intros Γ1 Γ2 Γ1' Γ2' ext_eq1 ext_eq2 step.
+    revert Γ1' Γ2' ext_eq1 ext_eq2. induction step; intros Γ1' Γ2' ext_eq1 ext_eq2.
+    - apply CtxtCommStep with (p := p) (q := q) (S := S) (T := T) (τ := τ).
+      1,2: rewrite <- ext_eq1; auto.
+      1,2: rewrite <- ext_eq2; auto.
+      intros r neq1 neq2; rewrite <- ext_eq1; rewrite <- ext_eq2; apply H3; auto.
+    - apply CtxtChoiceStep1 with (p := p) (q := q) (S := S) (T1 := T1) (T2 := T2).
+      1,2: rewrite <- ext_eq1; auto.
+      1,2: rewrite <- ext_eq2; auto.
+      intros r neq1 neq2; rewrite <- ext_eq1; rewrite <- ext_eq2; apply H3; auto.
+    - apply CtxtChoiceStep2 with (p := p) (q := q) (S := S) (T1 := T1) (T2 := T2).
+      1,2: rewrite <- ext_eq1; auto.
+      1,2: rewrite <- ext_eq2; auto.
+      intros r neq1 neq2; rewrite <- ext_eq1; rewrite <- ext_eq2; apply H3; auto.
+    - apply CtxtμStep with (p := p) (S := S).
+      rewrite <- ext_eq1; auto.
+      rewrite <- ext_eq2; auto.
+      intros r neq; rewrite <- ext_eq1; rewrite <- ext_eq2; apply H1; auto.
+  Qed.
+
+  Inductive CtxtStepMany : (Role -> SType) -> (Role -> SType) -> Prop :=
+    CtxtStepZero : forall Γ, CtxtStepMany Γ Γ
+  | CtxtStepMore : forall Γ1 Γ2 Γ3, CtxtStep Γ1 Γ2 -> CtxtStepMany Γ2 Γ3 -> CtxtStepMany Γ1 Γ3.
+
+  Inductive LiveContext : (Role -> SType) -> Prop :=
+    mkLive : forall Γ : Role -> SType,
+      (forall p q τ S, Γ p = SendType q τ S -> exists Γ', Γ' p = S /\ CtxtStepMany Γ Γ')
+      -> (forall p q τ S, Γ p = RecvType q τ S -> exists Γ', Γ' p = S /\ CtxtStepMany Γ Γ')
+      -> (forall p q S, Γ p = EChoiceType q S ->  exists Γ', Γ' p = S /\ CtxtStepMany Γ Γ')
+      -> (forall p q S1 S2, Γ p = IChoiceType q S1 S2 ->  exists Γ', Γ' p = S1 /\ CtxtStepMany Γ Γ')
+      -> (forall p q S1 S2, Γ p = IChoiceType q S1 S2 ->  exists Γ', Γ' p = S2 /\ CtxtStepMany Γ Γ')
+      -> (forall p S Γ', Γ p = μ S -> (forall r, p <> r -> Γ r = Γ' r) -> Γ' p = S [st| σμ S] -> LiveContext Γ')
+      -> (forall Γ', CtxtStep Γ Γ' -> LiveContext Γ')
+      -> LiveContext Γ.
+          
+  Definition LiveSend : forall Γ,
+      LiveContext Γ
+      -> forall p q τ S, Γ p = SendType q τ S -> exists Γ', Γ' p = S /\ CtxtStepMany Γ Γ' :=
+    fun Γ liveΓ =>
+      match liveΓ with
+      | mkLive Γ x x0 x1 x2 x3 x4 x5 => x
+      end.
+
+  Definition LiveRecv : forall Γ,
+      LiveContext Γ
+      -> forall p q τ S, Γ p = RecvType q τ S -> exists Γ', Γ' p = S /\ CtxtStepMany Γ Γ' :=
+    fun Γ liveΓ =>
+      match liveΓ with
+      | mkLive Γ x x0 x1 x2 x3 x4 x5 => x0
+      end.
+
+  Definition LiveEChoice : forall Γ,
+      LiveContext Γ
+      -> forall p q S, Γ p = EChoiceType q S ->  exists Γ', Γ' p = S /\ CtxtStepMany Γ Γ' :=
+    fun Γ liveΓ =>
+      match liveΓ with
+      | mkLive Γ x x0 x1 x2 x3 x4 x5 => x1
+      end.
+
+  Definition LiveIChoice1 : forall Γ,
+      LiveContext Γ
+      -> forall p q S1 S2, Γ p = IChoiceType q S1 S2 ->  exists Γ', Γ' p = S1 /\ CtxtStepMany Γ Γ' :=
+    fun Γ liveΓ =>
+      match liveΓ with
+      | mkLive Γ x x0 x1 x2 x3 x4 x5 => x2
+      end.
+  
+  Definition LiveIChoice2 : forall Γ,
+      LiveContext Γ
+      -> forall p q S1 S2, Γ p = IChoiceType q S1 S2 ->  exists Γ', Γ' p = S2 /\ CtxtStepMany Γ Γ' :=
+    fun Γ liveΓ =>
+      match liveΓ with
+      | mkLive Γ x x0 x1 x2 x3 x4 x5 => x3
+      end.
+
+  Definition Liveμ : forall Γ,
+      LiveContext Γ
+      -> forall p S Γ', Γ p = μ S -> (forall r, p <> r -> Γ r = Γ' r) -> Γ' p = S [st| σμ S] -> LiveContext Γ' :=
+    fun Γ liveΓ =>
+      match liveΓ with
+      | mkLive Γ x x0 x1 x2 x3 x4 x5 => x4
+      end.
+
+  Definition LiveStep : forall Γ,
+      LiveContext Γ
+      -> forall Γ', CtxtStep Γ Γ' -> LiveContext Γ' :=
+    fun Γ liveΓ =>
+      match liveΓ with
+      | mkLive Γ x x0 x1 x2 x3 x4 x5 => x5
+      end.
+
+  
